[MERGE] improve local inlining
commit f44672e21b3b373454237335fbf0f24ef385861d
Author: Basile Pesin <basile.pesin@vertmo.org>
Date:   Wed Jan 11 21:11:45 2023 +0100

    And fixed correctness proof

commit 5c8da0d7d82b0c20ce7fd4917e1d96514de22d7e
Author: Basile Pesin <basile.pesin@vertmo.org>
Date:   Wed Jan 11 10:23:10 2023 +0100

    Fixed typing proof

commit 1bf60482bec8289ae2e4b3d6470ad113346dbdb7
Author: Basile Pesin <basile.pesin@vertmo.org>
Date:   Tue Jan 10 19:35:53 2023 +0100

    Fixed clocking proof

commit c3ac5c0f43565a73fbd886bf738f6815edf13469
Author: Basile Pesin <basile.pesin@vertmo.org>
Date:   Tue Jan 10 11:37:29 2023 +0100

    Rewritten inlining of local blocks pass, proved node obligations

src/Lustre/InlineLocal/InlineLocal.v
@@ -107,65 +107,319 @@ Module Type INLINELOCAL
 
   Module Fresh := Fresh.Fresh(Ids).
   Import Fresh Notations Facts Tactics.
-  Local Open Scope fresh_monad_scope.
 
-  Definition FreshAnn A := Fresh local A (type * clock).
+  (* Be your own, personal, monad *)
+  Record reuse_st := {
+      fresh_st: fresh_st local unit; (* We dont actually need to keep type information in here *)
+      used: PS.t; (* Identifiers already used *)
+    }.
 
-  Fixpoint inlinelocal_block sub (blk : block) : FreshAnn (list block) :=
-    match blk with
-    | Beq eq => ret [Beq (rename_in_equation sub eq)]
-    | Breset blks er =>
-      do blks' <- mmap (inlinelocal_block sub) blks;
-      ret [Breset (concat blks') (rename_in_exp sub er)]
-    | Blocal (Scope locs blks) =>
-      let locs' := map (fun '(x, (ty, ck, _, _)) => (x, (ty, (rename_in_clock sub ck)))) locs in
-      do (_, sub1) <- fresh_idents_rename locs' (fun sub '(ty, ck) => (ty, rename_in_clock sub ck));
-      let sub' := Env.union sub sub1 in
-      do blks' <- mmap (inlinelocal_block sub') blks;
-      ret (concat blks')
-    | _ => (* Should not happen *) ret [blk]
+  Definition Reuse A := reuse_st -> (A * reuse_st).
+
+  Definition reuse_ident (x : ident) : Reuse ident :=
+    fun st =>
+      if PS.mem x st.(used) then
+        let (y, st') := fresh_ident (Some x) tt st.(fresh_st) in
+        (y, {| fresh_st := st'; used := st.(used) |})
+      else
+        (x, {| fresh_st := st.(fresh_st); used := PS.add x st.(used) |}).
+
+  Section ret.
+    Context {A : Type}.
+    Definition ret (x : A) : Reuse A := fun st => (x, st).
+
+    Fact ret_spec : forall a st,
+        ret a st = (a, st).
+    Proof.
+      intros a st. reflexivity.
+    Qed.
+  End ret.
+
+  Section bind.
+    Context {A B : Type}.
+    Definition bind (x : Reuse A) (k : A -> Reuse B) : Reuse B :=
+      fun st => let '(a, st') := x st in k a st'.
+
+    Lemma bind_spec : forall (x : Reuse A) (k : A -> Reuse B) st a' st'',
+        (bind x k) st = (a', st'') <->
+        exists a, exists st', (x st = (a, st') /\ k a st' = (a', st'')).
+    Proof.
+      intros x k st a' st''. split; intros.
+      - unfold bind in H.
+        destruct (x st) as [a st']. exists a. exists st'.
+        split; auto.
+      - destruct H as [a [st' [H1 H2]]]. unfold bind.
+        rewrite H1. assumption.
+    Qed.
+  End bind.
+
+  Section bind2.
+    Context {A1 A2 B : Type}.
+    Definition bind2 (x : Reuse (A1 * A2)) (k : A1 -> A2 -> Reuse B) : Reuse B :=
+      fun st => let '((a1, a2), st') := x st in k a1 a2 st'.
+
+    Lemma bind2_spec : forall (x : Reuse (A1 * A2)) (k : A1 -> A2 -> Reuse B) st a' st'',
+        (bind2 x k) st = (a', st'') <->
+          exists a1, exists a2, exists st', (x st = ((a1, a2), st') /\ k a1 a2 st' = (a', st'')).
+    Proof.
+      intros x k st a' st''. split; intros.
+      - unfold bind2 in H.
+        destruct (x st) as [[a1 a2] st']. exists a1. exists a2. exists st'.
+        split; auto.
+      - destruct H as [a1 [a2 [st' [H1 H2]]]]. unfold bind2.
+        rewrite H1. assumption.
+    Qed.
+  End bind2.
+
+  Definition st_In x (st : reuse_st) :=
+    In x (st_ids (fresh_st st)) \/ PS.In x (used st).
+
+  Definition st_valid (st : reuse_st) :=
+    PS.For_all (AtomOrGensym switch_prefs) (used st).
+
+  Definition st_follows (st1 st2 : reuse_st) :=
+    st_follows (fresh_st st1) (fresh_st st2) /\ PS.Subset (used st1) (used st2).
+
+  Global Instance st_follows_Reflexive : Reflexive st_follows.
+  Proof. split; reflexivity. Qed.
+  Global Instance st_follows_Transitive : Transitive st_follows.
+  Proof. intros ??? (?&?) (?&?). split; etransitivity; eauto. Qed.
+
+  Lemma st_follows_In : forall st1 st2,
+      st_follows st1 st2 ->
+      forall x, st_In x st1 -> st_In x st2.
+  Proof.
+    intros * (F1&F2) ? [In|In]; [left|right]; eauto.
+    eapply incl_map; eauto using st_follows_incl.
+  Qed.
+
+  Declare Scope reuse_monad_scope.
+  Notation "'do' X <- A ; B" :=
+    (bind A (fun X => B))
+      (at level 200, X name, A at level 100, B at level 200): reuse_monad_scope.
+  Notation "'do' ( X , Y ) <- A ; B" :=
+    (bind2 A (fun X Y => B))
+      (at level 200, X name, Y name, A at level 100, B at level 200): reuse_monad_scope.
+  Open Scope reuse_monad_scope.
+
+  Ltac monadInv :=
+    simpl in *;
+    match goal with
+    | H : context c [ret _ _] |- _ =>
+        rewrite ret_spec in H
+    | H : (_, _) = (_, _) |- _ =>
+        inv H
+    | H : bind _ _ _ = (_, _) |- _ =>
+        apply bind_spec in H; destruct H as [? [? [? ?]]]; simpl in *
+    | H : bind2 _ _ _ = (_, _) |- _ =>
+        apply bind2_spec in H; destruct H as [? [? [? [? ?]]]]; simpl in *
+    | |- context c [ret _ _] =>
+        rewrite ret_spec
+    | |- bind _ _ _ = (_, _) =>
+        rewrite bind_spec; repeat esplit
+    | |- bind2 _ _ _ = (_, _) =>
+        rewrite bind2_spec; repeat esplit
     end.
 
-  Definition inlinelocal_topblock (blk : block) : FreshAnn (list block * list (ident * _)) :=
+  Section mmap.
+    Context {A B : Type}.
+    Variable k : A -> Reuse B.
+    Fixpoint mmap a :=
+      match a with
+      | nil => ret nil
+      | hd::tl => do a1 <- k hd;
+                do a1s <- mmap tl;
+                ret (a1::a1s)
+      end.
+
+    Fact mmap_values : forall a st a1s st',
+        mmap a st = (a1s, st') ->
+        Forall2 (fun a a1 => exists st'', exists st''', k a st'' = (a1, st''')) a a1s.
+    Proof.
+      induction a; intros st a1s st' Hfold; simpl in *; repeat monadInv.
+      - constructor.
+      - specialize (IHa _ _ _ H0).
+        constructor; eauto.
+    Qed.
+
+    Fact mmap_st_valid : forall a a1s st st',
+        mmap a st = (a1s, st') ->
+        Forall (fun a => forall a1 st st', k a st = (a1, st') -> st_valid st -> st_valid st') a ->
+        st_valid st ->
+        st_valid st'.
+    Proof.
+      induction a; intros * Hmap F Val; inv F; repeat monadInv; eauto.
+    Qed.
+
+    Fact mmap_st_follows : forall a a1s st st',
+        mmap a st = (a1s, st') ->
+        Forall (fun a => forall a1 st st', k a st = (a1, st') -> st_follows st st') a ->
+        st_follows st st'.
+    Proof.
+      induction a; intros * Hmap F; inv F; repeat monadInv; auto.
+      - reflexivity.
+      - etransitivity; eauto.
+    Qed.
+
+    Fact mmap_values_follows : forall a st a1s st',
+        (forall a a1 st st', k a st = (a1, st') -> st_follows st st') ->
+        mmap a st = (a1s, st') ->
+        Forall2 (fun a a1 =>
+                   exists st'' st''',
+                     st_follows st st''
+                     /\ st_follows st''' st'
+                     /\ k a st'' = (a1, st''')) a a1s.
+    Proof.
+      induction a; intros * Follows Hfold; repeat monadInv.
+      - constructor.
+      - constructor.
+        + do 2 esplit; split; [|split]. 3:eauto. reflexivity.
+          eapply mmap_st_follows; eauto. simpl_Forall; eauto.
+        + eapply IHa in H0; eauto.
+          simpl_Forall.
+          do 2 esplit; split; [|split]. 3:eauto. 2:eauto. etransitivity; eauto.
+    Qed.
+
+    Fact mmap_values' : forall a st a1s st',
+        Forall (fun a => forall a1 st st', k a st = (a1, st') -> st_valid st -> st_valid st') a ->
+        (forall a a1 st st', k a st = (a1, st') -> st_follows st st') ->
+        mmap a st = (a1s, st') ->
+        st_valid st ->
+        Forall2 (fun a a1 =>
+                   exists st'' st''',
+                     st_valid st''
+                     /\ st_follows st st''
+                     /\ st_follows st''' st'
+                     /\ k a st'' = (a1, st''')) a a1s.
+    Proof.
+      induction a; intros * Valid Follows Hfold V; inv Valid; repeat monadInv.
+      - constructor.
+      - constructor.
+        + do 2 esplit; split; [|split; [|split]]. 1,4:eauto. reflexivity.
+          eapply mmap_st_follows; eauto. simpl_Forall; eauto.
+        + eapply IHa in H0; eauto.
+          simpl_Forall.
+          do 2 esplit; split; [|split; [|split]]. 1,4:eauto. 2:eauto. etransitivity; eauto.
+    Qed.
+  End mmap.
+
+  Section mmap2.
+    Context {A A1 A2 : Type}.
+    Variable k : A -> Reuse (A1 * A2).
+    Fixpoint mmap2 (a : list A) : Reuse (list A1 * list A2) :=
+      match a with
+      | nil => ret (nil, nil)
+      | hd::tl => do (a1, a2) <- k hd;
+                do (a1s, a2s) <- mmap2 tl;
+                ret (a1::a1s, a2::a2s)
+      end.
+
+    Fact mmap2_values : forall a st a1s a2s st',
+        mmap2 a st = (a1s, a2s, st') ->
+        Forall3 (fun a a1 a2 => exists st'', exists st''', k a st'' = (a1, a2, st''')) a a1s a2s.
+    Proof.
+      induction a; intros st a1s a2s st' Hfold; simpl in *; repeat monadInv.
+      - constructor.
+      - specialize (IHa _ _ _ _ H0).
+        constructor; eauto.
+    Qed.
+
+    Fact mmap2_st_valid : forall a a1s a2s st st',
+        mmap2 a st = (a1s, a2s, st') ->
+        Forall (fun a => forall a1 a2 st st', k a st = (a1, a2, st') -> st_valid st -> st_valid st') a ->
+        st_valid st ->
+        st_valid st'.
+    Proof.
+      induction a; intros a1s a2s st st' Hmap F; inv F; repeat monadInv; eauto.
+    Qed.
+
+    Fact mmap2_st_follows : forall a a1s a2s st st',
+        mmap2 a st = (a1s, a2s, st') ->
+        Forall (fun a => forall a1 a2 st st', k a st = (a1, a2, st') -> st_follows st st') a ->
+        st_follows st st'.
+    Proof.
+      induction a; intros a1s a2s st st' Hmap F; inv F; repeat monadInv.
+      - reflexivity.
+      - etransitivity; eauto.
+    Qed.
+
+    Fact mmap2_values_follows : forall a st a1s a2s st',
+        (forall a a1 a2 st st', k a st = (a1, a2, st') -> st_follows st st') ->
+        mmap2 a st = (a1s, a2s, st') ->
+        Forall3 (fun a a1 a2 =>
+                   exists st'' st''',
+                     st_follows st st''
+                     /\ st_follows st''' st'
+                     /\ k a st'' = (a1, a2, st''')) a a1s a2s.
+    Proof.
+      induction a; intros * Follows Hfold; simpl in *; repeat monadInv.
+      - constructor.
+      - constructor.
+        + do 2 esplit; split; [|split]. 3:eauto. reflexivity.
+          eapply mmap2_st_follows; eauto. simpl_Forall; eauto.
+        + eapply IHa in H0; eauto.
+          eapply Forall3_impl_In; [|eauto]. intros; destruct_conjs.
+          do 2 esplit; split; [|split]. 3:eauto. 2:eauto. etransitivity; eauto.
+    Qed.
+
+    Fact mmap2_values' : forall a st a1s a2s st',
+        Forall (fun a => forall a1 a2 st st', k a st = (a1, a2, st') -> st_valid st -> st_valid st') a ->
+        (forall a a1 a2 st st', k a st = (a1, a2, st') -> st_follows st st') ->
+        mmap2 a st = (a1s, a2s, st') ->
+        st_valid st ->
+        Forall3 (fun a a1 a2 =>
+                   exists st'' st''',
+                     st_valid st''
+                     /\ st_follows st st''
+                     /\ st_follows st''' st'
+                     /\ k a st'' = (a1, a2, st''')) a a1s a2s.
+    Proof.
+      induction a; intros * Valid Follows Hfold V; inv Valid; repeat monadInv.
+      - constructor.
+      - constructor.
+        + do 2 esplit; split; [|split; [|split]]. 1,4:eauto. reflexivity.
+          eapply mmap2_st_follows; eauto. simpl_Forall; eauto.
+        + eapply IHa in H0; eauto.
+          eapply Forall3_impl_In; [|eauto]. intros; destruct_conjs.
+          do 2 esplit; split; [|split; [|split]]. 1,4:eauto. 2:eauto. etransitivity; eauto.
+    Qed.
+  End mmap2.
+
+  Fixpoint inlinelocal_block sub (blk : block) : Reuse (list (ident * ann) * list block) :=
     match blk with
+    | Beq eq => ret ([], [Beq (rename_in_equation sub eq)])
+    | Breset blks er =>
+        do (locs, blks') <- mmap2 (inlinelocal_block sub) blks;
+        ret (concat locs, [Breset (concat blks') (rename_in_exp sub er)])
     | Blocal (Scope locs blks) =>
-      do blks' <- mmap (inlinelocal_block (@Env.empty _)) blks;
-      ret (concat blks', locs)
-    | _ =>
-      do blks' <- inlinelocal_block (@Env.empty _) blk;
-      ret (blks', [])
+        let xs := map fst locs in
+        do newlocs <- mmap reuse_ident xs;
+        let sub1 := Env.from_list (combine xs newlocs) in
+        let sub' := Env.union sub sub1 in
+        let locs' := map (fun '(x, (ty, ck, _, _)) => (rename_var sub' x, (ty, (rename_in_clock sub' ck)))) locs in
+        do (locs1, blks') <- mmap2 (inlinelocal_block sub') blks;
+        ret (locs'++concat locs1, concat blks')
+    | _ => (* Should not happen *) ret ([], [blk])
     end.
 
   (** ** State properties *)
 
-  Lemma inlinelocal_block_st_follows : forall blk sub blks' st st',
-      inlinelocal_block sub blk st = (blks', st') ->
-      st_follows st st'.
-  Proof.
-    induction blk using block_ind2; intros * Hdl; repeat inv_bind; try reflexivity.
-    - (* reset *)
-      eapply mmap_st_follows in H0; eauto.
-      rewrite Forall_forall in *; eauto.
-    - (* local *)
-      eapply fresh_idents_rename_st_follows in H0; eauto.
-      etransitivity; eauto.
-      eapply mmap_st_follows in H1; eauto.
-      rewrite Forall_forall in *; eauto.
-  Qed.
+  (* Lemma inlinelocal_block_st_follows : forall blk sub blks' st st', *)
+  (*     inlinelocal_block sub blk st = (blks', st') -> *)
+  (*     st_follows st st'. *)
+  (* Proof. *)
+  (*   induction blk using block_ind2; intros * Hdl; repeat inv_bind; try reflexivity. *)
+  (*   - (* reset *) *)
+  (*     eapply mmap_st_follows in H0; eauto. *)
+  (*     rewrite Forall_forall in *; eauto. *)
+  (*   - (* local *) *)
+  (*     eapply fresh_idents_rename_st_follows in H0; eauto. *)
+  (*     etransitivity; eauto. *)
+  (*     eapply mmap_st_follows in H1; eauto. *)
+  (*     rewrite Forall_forall in *; eauto. *)
+  (* Qed. *)
 
-  Lemma inlinelocal_topblock_st_follows : forall blk res st st',
-      inlinelocal_topblock blk st = (res, st') ->
-      st_follows st st'.
-  Proof.
-    Opaque inlinelocal_block.
-    destruct blk; intros * Hil; try destruct s; repeat inv_bind.
-    1-4:eapply inlinelocal_block_st_follows; eauto.
-    eapply mmap_st_follows; eauto.
-    eapply Forall_forall; intros; eauto using inlinelocal_block_st_follows.
-    Transparent inlinelocal_block.
-  Qed.
-
-  Global Hint Resolve inlinelocal_block_st_follows : fresh.
+  (* Global Hint Resolve inlinelocal_block_st_follows : fresh. *)
 
   (** ** Wellformedness properties *)
 
@@ -173,155 +427,244 @@ Module Type INLINELOCAL
 
   Import Permutation.
 
-  Fact mmap_vars_perm : forall (f : _ -> block -> FreshAnn (list block)) blks sub blks' xs st st',
+  Fact mmap_vars_perm : forall (f : _ -> block -> Reuse (list (ident * ann) * list block)) blks sub locs' blks' xs st st',
       Forall
-        (fun blk => forall sub blks' xs st st',
+        (fun blk => forall sub locs' blks' xs st st',
              noswitch_block blk ->
              VarsDefined blk xs ->
              NoDupLocals (map fst (Env.elements sub) ++ xs) blk ->
-             f sub blk st = (blks', st') ->
-             exists ys, Forall2 VarsDefined blks' ys /\ Permutation (concat ys ++ st_ids st) (map (rename_var sub) xs ++ st_ids st')) blks ->
+             f sub blk st = (locs', blks', st') ->
+             exists ys, Forall2 VarsDefined blks' ys /\ Permutation (concat ys) (map (rename_var sub) xs ++ map fst locs')) blks ->
       Forall noswitch_block blks ->
       Forall2 VarsDefined blks xs ->
       Forall (NoDupLocals (map fst (Env.elements sub) ++ concat xs)) blks ->
-      mmap (f sub) blks st = (blks', st') ->
-      exists ys, Forall2 VarsDefined (concat blks') ys /\ Permutation (concat ys ++ st_ids st) (map (rename_var sub) (concat xs) ++ st_ids st').
+      mmap2 (f sub) blks st = (locs', blks', st') ->
+      exists ys, Forall2 VarsDefined (concat blks') ys /\ Permutation (concat ys) (map (rename_var sub) (concat xs) ++ map fst (concat locs')).
   Proof.
-    induction blks; intros * Hf Hns Hvars Hnd Hnorm; inv Hf; inv Hns; inv Hvars; inv Hnd; repeat inv_bind; simpl.
+    induction blks; intros * Hf Hns Hvars Hnd Hnorm; inv Hf; inv Hns; inv Hvars; inv Hnd; repeat monadInv; simpl.
     - exists []. split; auto.
     - eapply H1 in H as (ys1&Hvars1&Hperm1); eauto.
       2:eapply NoDupLocals_incl; [|eauto]; solve_incl_app.
       eapply IHblks in H2 as (ys2&Hvars2&Hperm2); eauto. clear IHblks.
-      2:eapply Forall_impl; [|eapply H8]; intros; eapply NoDupLocals_incl; [|eauto]; solve_incl_app.
+      2:simpl_Forall; intros; eapply NoDupLocals_incl; [|eauto]; solve_incl_app.
       exists (ys1 ++ ys2). split.
       + apply Forall2_app; auto.
-      + rewrite map_app, <-app_assoc, <-Hperm2, Permutation_swap, <-Hperm1, Permutation_swap.
-        now rewrite concat_app, <-app_assoc.
+      + rewrite concat_app, Hperm1, Hperm2. solve_Permutation_app.
   Qed.
 
-  Lemma inlinelocal_block_vars_perm : forall blk sub blks' xs st st',
+  Lemma inlinelocal_block_vars_perm : forall blk sub locs' blks' xs st st',
       noswitch_block blk ->
       VarsDefined blk xs ->
       NoDupLocals (map fst (Env.elements sub) ++ xs) blk ->
-      inlinelocal_block sub blk st = (blks', st') ->
-      exists ys, Forall2 VarsDefined blks' ys /\ Permutation (concat ys ++ st_ids st) (map (rename_var sub) xs ++ st_ids st').
+      inlinelocal_block sub blk st = (locs', blks', st') ->
+      exists ys, Forall2 VarsDefined blks' ys /\ Permutation (concat ys) (map (rename_var sub) xs ++ map fst locs').
   Proof.
     induction blk using block_ind2; intros * Hns Hvars Hnd Hdl;
-      inv Hns; inv Hvars; inv Hnd; repeat inv_bind.
+      inv Hns; inv Hvars; inv Hnd; repeat monadInv.
     - (* equation *)
       destruct eq.
       repeat esplit; simpl; eauto using VarsDefined with datatypes.
-      simpl. now rewrite <-app_assoc.
     - (* reset *)
       eapply mmap_vars_perm in H0 as (ys1&Hvars1&Hperm1); eauto.
       do 2 esplit; eauto using VarsDefined.
-      simpl. now rewrite <-app_assoc.
+      simpl. now rewrite app_nil_r.
     - (* local *)
-      inv H1. inv H5. inv_VarsDefined.
+      repeat inv_scope. take (Permutation _ _) and rename it into Hperm.
       eapply mmap_vars_perm in H4 as (ys1&Hvars1&Hperm1); eauto.
       2:{ simpl_Forall.
           eapply NoDupLocals_incl; [|eauto].
-          rewrite <-app_assoc, <-Hperm.
+          rewrite <-app_assoc, Hperm.
           apply incl_app; try solve [solve_incl_app].
           intros ? Hin. simpl_In.
           eapply Env.elements_complete, Env.union_find4 in Hin0 as [Hfind|Hfind].
           - eapply Env.elements_correct in Hfind.
             apply in_or_app, or_introl; solve_In.
-          - eapply fresh_idents_rename_sub1 in H0; eauto. 2:econstructor; eauto.
-            rewrite fst_InMembers in H0. simpl_In.
-            rewrite Hperm, 2 in_app_iff. right; right. solve_In.
+          - eapply Env.from_list_find_In, in_combine_l in Hfind.
+            rewrite 2 in_app_iff. auto.
       }
       rewrite Hperm, map_app in Hperm1.
-      unfold st_ids in Hperm1. do 1 (erewrite fresh_idents_rename_anns in Hperm1; eauto); simpl in *.
-      do 2 esplit; eauto.
-      rewrite map_app, not_in_union_map_rename2, not_in_union_map_rename1,
-        (Permutation_swap (concat ys1)), <-app_assoc in Hperm1.
-      2:{ simpl_Forall; subst.
-          intros (?&contra). eapply H11; eauto using In_InMembers.
-          apply in_or_app; left. solve_In.
-          2:eapply Env.elements_correct; eauto. reflexivity. }
-      2:{ simpl_Forall; subst.
-          intro contra. eapply fresh_idents_rename_sub1 in contra; eauto.
-          rewrite fst_InMembers in contra; simpl_In.
-          eapply H11; eauto using In_InMembers, in_or_app. }
-      eapply Ker.fresh_idents_rename_ids in H0.
-      2:{ apply NoDupMembers_map; auto. intros; destruct_conjs; auto. }
-      rewrite H0 in Hperm1. repeat rewrite map_map in Hperm1; simpl in Hperm1.
-      rewrite Permutation_swap with (xs:=map _ xs) in Hperm1.
-      erewrite map_ext in Hperm1. eapply Permutation_app_inv_l in Hperm1; auto.
-      intros; destruct_conjs; auto.
+      do 2 esplit; eauto. rewrite Hperm1, map_app, 2 map_map, <-app_assoc.
+      erewrite not_in_union_map_rename2, map_ext with (l:=locs). reflexivity.
+      + intros; destruct_conjs. reflexivity.
+      + simpl_Forall. intros In.
+        eapply Env.In_from_list, InMembers_In_combine, fst_InMembers in In.
+        eapply H12; eauto with datatypes.
   Qed.
 
-  Lemma inlinelocal_topblock_vars_perm : forall blk blks' vars xs st st',
-      noswitch_block blk ->
-      VarsDefined blk xs ->
-      NoDupLocals xs blk ->
-      inlinelocal_topblock blk st = (blks', vars, st') ->
-      exists ys, Forall2 VarsDefined blks' ys /\ Permutation (concat ys ++ st_ids st) (xs ++ map fst vars ++ st_ids st').
+  (** *** st_valid *)
+
+  Lemma reuse_ident_st_valid : forall x y st st',
+      AtomOrGensym switch_prefs x ->
+      reuse_ident x st = (y, st') ->
+      st_valid st ->
+      st_valid st'.
   Proof.
-    Opaque inlinelocal_block.
-    destruct blk; intros * Hns Hvars Hnd Hil; try destruct s; repeat inv_bind; simpl.
-    1-4:eapply inlinelocal_block_vars_perm in H as (?&?&Hperm); eauto.
-    5:(inv Hvars; inv Hnd;
-       take (VarsDefinedScope _ _ _) and inv it; inv_VarsDefined;
-       take (NoDupScope _ _ _) and inv it; eapply mmap_vars_perm in H as (?&?&Hperm'); eauto).
-    1-5:try rewrite rename_vars_empty in Hperm; eauto.
-    - rewrite rename_vars_empty in Hperm'; eauto.
-      do 2 esplit; eauto. rewrite Hperm', Hperm, <-app_assoc; auto.
-    - eapply Forall_forall; intros; eauto using inlinelocal_block_vars_perm.
-    - inv Hns; auto.
-    - rewrite Env.Props.P.elements_empty; simpl.
-      eapply Forall_impl; [|eauto]; intros.
-      now rewrite Hperm.
-    Transparent inlinelocal_block.
+    intros * At Reu V. unfold reuse_ident in *.
+    cases_eqn EQ; inv_equalities; simpl.
+    apply PS_For_all_add. split; auto.
+  Qed.
+
+  Corollary reuse_idents_st_valid : forall locs locs' st st',
+      Forall (AtomOrGensym switch_prefs) locs ->
+      mmap reuse_ident locs st = (locs', st') ->
+      st_valid st ->
+      st_valid st'.
+  Proof.
+    intros * At Map V.
+    eapply mmap_st_valid; eauto. simpl_Forall; eauto using reuse_ident_st_valid.
+  Qed.
+
+  Lemma inlinelocal_block_st_valid : forall blk sub locs' blks' st st',
+      GoodLocals switch_prefs blk ->
+      inlinelocal_block sub blk st = (locs', blks', st') ->
+      st_valid st ->
+      st_valid st'.
+  Proof.
+    induction blk using block_ind2; intros * Good Il V; inv Good;
+      repeat monadInv; auto.
+    - (* reset *)
+      eapply mmap2_st_valid; eauto.
+      simpl_Forall; eauto.
+    - (* local *)
+      repeat inv_scope.
+      eapply mmap2_st_valid; eauto using reuse_idents_st_valid. simpl_Forall; eauto.
+  Qed.
+
+  (** *** st_follows *)
+
+  Lemma reuse_ident_st_follows : forall x y st st',
+      reuse_ident x st = (y, st') ->
+      st_follows st st'.
+  Proof.
+    intros * Reu. unfold reuse_ident in *.
+    cases_eqn EQ; inv_equalities; split; try reflexivity; simpl.
+    - eauto using fresh_ident_st_follows.
+    - intros ??; eauto using PSF.add_2.
+  Qed.
+
+  Lemma inlinelocal_block_st_follows : forall blk sub locs' blks' st st',
+      inlinelocal_block sub blk st = (locs', blks', st') ->
+      st_follows st st'.
+  Proof.
+    induction blk using block_ind2; intros * Il; repeat monadInv; try reflexivity.
+    - (* reset *)
+      eapply mmap2_st_follows; eauto.
+      simpl_Forall; eauto.
+    - (* local *)
+      etransitivity.
+      + eapply mmap_st_follows; eauto. simpl_Forall; eauto using reuse_ident_st_follows.
+      + eapply mmap2_st_follows; eauto.
+        simpl_Forall; eauto.
   Qed.
 
   (** *** GoodLocals *)
 
-  Lemma inlinelocal_block_GoodLocals : forall blk sub blks' st st',
+  Lemma inlinelocal_block_GoodLocals : forall blk sub blks' locs' st st',
       noswitch_block blk ->
-      inlinelocal_block sub blk st = (blks', st') ->
+      inlinelocal_block sub blk st = (locs', blks', st') ->
       Forall (GoodLocals local_prefs) blks'.
   Proof.
-    induction blk using block_ind2; intros * Hns Hdl; inv Hns; repeat inv_bind.
+    induction blk using block_ind2; intros * Hns Hdl; inv Hns; repeat monadInv.
     - (* equation *)
       repeat constructor.
     - (* reset *)
       repeat constructor. apply Forall_concat.
-      eapply mmap_values, Forall2_ignore1 in H0.
-      rewrite Forall_forall in *; intros * Hin.
-      edestruct H0 as (?&Hin'&?&?&Hdl); eauto.
+      eapply mmap2_values, Forall3_ignore12 in H0. simpl_Forall.
+      eapply H in H4; eauto. simpl_Forall; auto.
     - (* local *)
       apply Forall_concat.
-      eapply mmap_values, Forall2_ignore1 in H1.
-      rewrite Forall_forall in *; intros * Hin.
-      edestruct H1 as (?&Hin'&?&?&Hdl); eauto.
+      eapply mmap2_values, Forall3_ignore12 in H1. simpl_Forall.
+      eapply H in H6; eauto. simpl_Forall; auto.
   Qed.
 
-  Lemma inlinelocal_topblock_GoodLocals : forall blk blks' vars st st',
-      noswitch_block blk ->
-      inlinelocal_topblock blk st = (blks', vars, st') ->
-      Forall (GoodLocals local_prefs) blks'.
+  Lemma reuse_idents_find {A} : forall (locs: list (ident * A)) locs' st st' x,
+      NoDupMembers locs ->
+      mmap reuse_ident (map fst locs) st = (locs', st') ->
+      InMembers x locs ->
+      exists st st' y,
+        reuse_ident x st = (y, st')
+        /\ Env.find x (Env.from_list (combine (map fst locs) locs')) = Some y.
   Proof.
-    Opaque inlinelocal_block.
-    destruct blk; intros * Hns Hil; try destruct s; repeat inv_bind.
-    1-4:eapply inlinelocal_block_GoodLocals; eauto.
-    apply Forall_concat.
-    eapply mmap_values, Forall2_ignore1 in H. inv Hns.
-    rewrite Forall_forall in *; intros * Hin.
-    edestruct H as (?&Hin'&?&?&Hdl); eauto using inlinelocal_block_GoodLocals.
-    Transparent inlinelocal_block.
+    intros * ND Reuse In. apply fst_InMembers in In.
+    eapply mmap_values, Forall2_forall2 in Reuse as (Len&Nth).
+    eapply In_nth with (d:=xH) in In as (?&N&NthLocs); subst.
+    setoid_rewrite Env.find_In_from_list.
+    3:now apply NoDup_NoDupMembers_combine, fst_NoDupMembers.
+    2:{ erewrite <-combine_nth; [|eauto].
+        eapply nth_In with (d:=(xH, xH)). now rewrite combine_length, <-Len, Nat.min_id. }
+    specialize (Nth xH xH _ _ _ N eq_refl eq_refl) as (?&?&?).
+    do 2 esplit; eauto.
   Qed.
 
-  Lemma inlinelocal_topblock_AtomOrGensym : forall blk blks' vars st st',
+  Lemma reuse_idents_find_follows {A} : forall (locs: list (ident * A)) locs' st st' x,
+      NoDupMembers locs ->
+      mmap reuse_ident (map fst locs) st = (locs', st') ->
+      InMembers x locs ->
+      exists st1 st1' y,
+        st_follows st st1
+        /\ st_follows st1' st'
+        /\ reuse_ident x st1 = (y, st1')
+        /\ Env.find x (Env.from_list (combine (map fst locs) locs')) = Some y.
+  Proof.
+    intros * ND Reuse In. apply fst_InMembers in In.
+    eapply mmap_values_follows, Forall2_forall2 in Reuse as (Len&Nth); eauto using reuse_ident_st_follows.
+    eapply In_nth with (d:=xH) in In as (?&N&NthLocs); subst.
+    setoid_rewrite Env.find_In_from_list.
+    3:now apply NoDup_NoDupMembers_combine, fst_NoDupMembers.
+    2:{ erewrite <-combine_nth; [|eauto].
+        eapply nth_In with (d:=(xH, xH)). now rewrite combine_length, <-Len, Nat.min_id. }
+    specialize (Nth xH xH _ _ _ N eq_refl eq_refl) as (?&?&?&?&?).
+    do 2 esplit; eauto.
+  Qed.
+
+  Lemma reuse_idents_find' {A} : forall (locs: list (ident * A)) locs' st st' x,
+      NoDupMembers locs ->
+      Forall (AtomOrGensym switch_prefs) (map fst locs) ->
+      mmap reuse_ident (map fst locs) st = (locs', st') ->
+      st_valid st ->
+      InMembers x locs ->
+      exists st1 st1' y,
+        st_valid st1
+        /\ st_follows st st1
+        /\ st_follows st1' st'
+        /\ reuse_ident x st1 = (y, st1')
+        /\ Env.find x (Env.from_list (combine (map fst locs) locs')) = Some y.
+  Proof.
+    intros * ND At Reuse V In. apply fst_InMembers in In.
+    eapply mmap_values', Forall2_forall2 in Reuse as (Len&Nth); eauto using reuse_ident_st_follows.
+    2:{ clear In. simpl_Forall; eauto using reuse_ident_st_valid. }
+    eapply In_nth with (d:=xH) in In as (?&N&NthLocs); subst.
+    setoid_rewrite Env.find_In_from_list.
+    3:now apply NoDup_NoDupMembers_combine, fst_NoDupMembers.
+    2:{ erewrite <-combine_nth; [|eauto].
+        eapply nth_In with (d:=(xH, xH)). now rewrite combine_length, <-Len, Nat.min_id. }
+    specialize (Nth xH xH _ _ _ N eq_refl eq_refl) as (?&?&?&?&?&?).
+    do 2 esplit; eauto 6.
+  Qed.
+
+  Lemma inlinelocal_block_AtomOrGensym : forall blk Γ sub blks' locs' st st',
+      NoDupLocals Γ blk ->
       GoodLocals switch_prefs blk ->
-      inlinelocal_topblock blk st = (blks', vars, st') ->
-      Forall (AtomOrGensym switch_prefs) (map fst vars).
+      inlinelocal_block sub blk st = (locs', blks', st') ->
+      Forall (fun '(x, _) => AtomOrGensym local_prefs x) locs'.
   Proof.
-    Opaque inlinelocal_block.
-    destruct blk; intros * Hgood Hil; try destruct s; repeat inv_bind; try constructor.
-    inv Hgood. inv H1; eauto.
-    Transparent inlinelocal_block.
+    induction blk using block_ind2; intros * ND Good Hdl; inv ND; inv Good; repeat monadInv; try constructor.
+    - (* reset *)
+      apply Forall_concat.
+      eapply mmap2_values, Forall3_ignore13 in H0. simpl_Forall.
+      eapply H in H5; eauto. simpl_Forall; auto.
+    - (* local *)
+      repeat inv_scope.
+      apply Forall_app; split.
+      + simpl_Forall. eapply reuse_idents_find in H0 as (?&?&?&Reu&Find); eauto using In_InMembers.
+        unfold rename_var. erewrite Env.union_find3'; eauto. simpl.
+        unfold reuse_ident in Reu. cases_eqn EQ; inv_equalities.
+        * eapply fresh_ident_prefixed in EQ0 as (?&?&?); subst.
+          right. do 2 esplit; eauto using PSF.add_1.
+        * eauto using AtomOrGensym_add.
+      + apply Forall_concat.
+        eapply mmap2_values, Forall3_ignore13 in H3. simpl_Forall.
+        eapply H in H4; eauto. simpl_Forall; auto.
   Qed.
 
   (** *** NoDupLocals *)
@@ -339,110 +682,21 @@ Module Type INLINELOCAL
     eapply NoDup_snd_det; eauto using Env.elements_correct.
   Qed.
 
-  Lemma inlinelocal_block_NoDupLocals xs : forall blk sub blks' st st',
+  Lemma inlinelocal_block_NoDupLocals xs : forall blk sub locs' blks' st st',
       noswitch_block blk ->
-      inlinelocal_block sub blk st = (blks', st') ->
+      inlinelocal_block sub blk st = (locs', blks', st') ->
       Forall (NoDupLocals xs) blks'.
   Proof.
-    induction blk using block_ind2; intros * Hns Hdl; inv Hns; repeat inv_bind.
-    - (* equation *)
-      repeat constructor.
+    induction blk using block_ind2; intros * Hns Hdl; inv Hns; repeat monadInv; repeat constructor.
     - (* reset *)
-      repeat constructor.
-      eapply mmap_values, Forall2_ignore1 in H0.
-      eapply Forall_concat. rewrite Forall_forall in *; intros.
-      edestruct H0 as (?&?&?&?&?); eauto.
+      eapply mmap2_values, Forall3_ignore12 in H0.
+      eapply Forall_concat. simpl_Forall.
+      eapply H in H4; eauto. now simpl_Forall.
     - (* local *)
-      eapply mmap_values, Forall2_ignore1 in H1.
-      eapply Forall_concat. rewrite Forall_forall in *; intros.
-      edestruct H1 as (?&?&?&?&?); eauto.
+      eapply mmap2_values, Forall3_ignore12 in H1.
+      eapply Forall_concat. simpl_Forall.
+      eapply H in H6; eauto. now simpl_Forall.
   Qed.
-
-  Lemma inlinelocal_topblock_NoDupLocals xs : forall blk blks' vars st st',
-      noswitch_block blk ->
-      inlinelocal_topblock blk st = (blks', vars, st') ->
-      Forall (NoDupLocals xs) blks'.
-  Proof.
-    Opaque inlinelocal_block.
-    destruct blk; intros * Hns Hil; try destruct s; repeat inv_bind.
-    1-4:eapply inlinelocal_block_NoDupLocals; eauto.
-    eapply mmap_values, Forall2_ignore1 in H. inv Hns.
-    eapply Forall_concat. rewrite Forall_forall in *; intros.
-    edestruct H as (?&?&?&?&?); eauto using inlinelocal_block_NoDupLocals.
-    Transparent inlinelocal_block.
-  Qed.
-
-  Lemma inlinelocal_topblock_NoDupMembers xs : forall blk blks' vars st st',
-      NoDupLocals xs blk ->
-      inlinelocal_topblock blk st = (blks', vars, st') ->
-      NoDupMembers vars.
-  Proof.
-    Opaque inlinelocal_block.
-    destruct blk; intros * Hnd Hil; inv Hnd; try destruct s; repeat inv_bind; auto.
-    1-4:constructor.
-    inv H1; auto.
-    Transparent inlinelocal_block.
-  Qed.
-
-  Lemma inlinelocal_topblock_nIn xs : forall blk blks' vars st st',
-      NoDupLocals xs blk ->
-      inlinelocal_topblock blk st = (blks', vars, st') ->
-      forall x, InMembers x vars -> ~In x xs.
-  Proof.
-    Opaque inlinelocal_block.
-    destruct blk; intros * Hnd Hil; inv Hnd; try destruct s; repeat inv_bind; auto.
-    inv H1; auto.
-    Transparent inlinelocal_block.
-  Qed.
-
-  (** *** No local block *)
-
-  Lemma inlinelocal_block_nolocal : forall blk sub blks' st st',
-      noswitch_block blk ->
-      inlinelocal_block sub blk st = (blks', st') ->
-      Forall nolocal_block blks'.
-  Proof.
-    induction blk using block_ind2; intros * Hns Hdl; inv Hns; repeat inv_bind.
-    - (* equation *)
-      repeat constructor.
-    - (* reset *)
-      repeat constructor.
-      eapply mmap_values, Forall2_ignore1 in H0.
-      eapply Forall_concat.
-      rewrite Forall_forall in *; intros.
-      edestruct H0 as (?&?&(?&?&?)); eauto.
-    - (* local *)
-      eapply mmap_values, Forall2_ignore1 in H1.
-      eapply Forall_concat.
-      rewrite Forall_forall in *; intros.
-      edestruct H1 as (?&?&?&?&Hdl); eauto.
-  Qed.
-
-  Lemma inlinelocal_topblock_nolocal : forall blk blks' vars st st',
-      noswitch_block blk ->
-      inlinelocal_topblock blk st = (blks', vars, st') ->
-      Forall nolocal_block blks'.
-  Proof.
-    Opaque inlinelocal_block.
-    destruct blk; intros * Hns Hil; try destruct s; repeat inv_bind.
-    1-4:eapply inlinelocal_block_nolocal; eauto.
-    eapply mmap_values, Forall2_ignore1 in H. inv Hns.
-    eapply Forall_concat.
-    rewrite Forall_forall in *; intros.
-    edestruct H as (?&?&?&?&Hdl); eauto using inlinelocal_block_nolocal.
-    Transparent inlinelocal_block.
-  Qed.
-
-  Lemma inlinelocal_topblock_nolast : forall blk blks' vars st st',
-      noswitch_block blk ->
-      inlinelocal_topblock blk st = (blks', vars, st') ->
-      Forall (fun '(_, (_, _, _, o)) => o = None) vars.
-  Proof.
-    intros * Hns Hil.
-    inv Hns; repeat inv_bind; auto.
-  Qed.
-
-  (** ** Transformation of node and program *)
 
   Lemma local_not_in_switch_prefs :
     ~PS.In local switch_prefs.
@@ -454,8 +708,262 @@ Module Type INLINELOCAL
     intros [contra|[contra|[contra|contra]]]; subst; rewrite contra in *; eauto 10 with datatypes.
   Qed.
 
+  Lemma reuse_ident_In : forall x y st st',
+      reuse_ident x st = (y, st') ->
+      PS.In x (used st').
+  Proof.
+    intros * Reu. unfold reuse_ident in *.
+    cases_eqn EQ.
+    inv Reu; eauto using PSF.add_1.
+  Qed.
+
+  Corollary reuse_idents_In : forall locs locs' st st',
+    mmap reuse_ident locs st = (locs', st') ->
+    Forall (fun x => PS.In x (used st')) locs.
+  Proof.
+    intros * Reu.
+    eapply mmap_values_follows, Forall2_ignore2 in Reu; eauto using reuse_ident_st_follows.
+    simpl_Forall.
+    eapply H2, reuse_ident_In; eauto.
+  Qed.
+
+  Lemma reuse_ident_st_In : forall x y st st',
+      reuse_ident x st = (y, st') ->
+      st_In y st'.
+  Proof.
+    intros * Reu. unfold reuse_ident in *.
+    cases_eqn EQ; inv_equalities.
+    - left. eapply fresh_ident_Inids; eauto.
+    - right. eauto using PSF.add_1.
+  Qed.
+
+  Corollary reuse_idents_st_In : forall locs locs' st st',
+    mmap reuse_ident locs st = (locs', st') ->
+    Forall (fun x => st_In x st') locs'.
+  Proof.
+    intros * Reu.
+    eapply mmap_values_follows, Forall2_ignore1 in Reu; eauto using reuse_ident_st_follows.
+    simpl_Forall.
+    eapply reuse_ident_st_In in H3; eauto using st_follows_In.
+  Qed.
+
+  Lemma inlinelocal_block_st_In : forall blk Γ sub blks' locs' st st',
+      NoDupLocals Γ blk ->
+      inlinelocal_block sub blk st = (locs', blks', st') ->
+      Forall (fun '(x, _) => st_In x st') locs'.
+  Proof.
+    induction blk using block_ind2; intros * ND IL; inv ND;
+      repeat monadInv; try constructor.
+    - (* reset *)
+      eapply mmap2_values_follows, Forall3_ignore13 in H0; eauto using inlinelocal_block_st_follows.
+      apply Forall_concat. simpl_Forall.
+      eapply H in H6; eauto. simpl_Forall; eauto using st_follows_In.
+    - (* local *)
+      inv H2.
+      apply Forall_app; split.
+      + simpl_Forall.
+        eapply reuse_idents_find_follows in H0 as (?&?&?&F1&F2&Reu&Find); eauto using In_InMembers.
+        unfold rename_var. erewrite Env.union_find3'; eauto. simpl.
+        eapply reuse_ident_st_In in Reu. eapply st_follows_In; [|eauto].
+        etransitivity; eauto. eapply mmap2_st_follows; eauto. simpl_Forall; eauto using inlinelocal_block_st_follows.
+      + eapply mmap2_values_follows, Forall3_ignore13 in H1; eauto using inlinelocal_block_st_follows.
+        apply Forall_concat. simpl_Forall.
+        eapply H in H9; eauto. simpl_Forall. eauto using st_follows_In.
+  Qed.
+
+  Lemma reuse_ident_st_nIn : forall x y st st',
+      AtomOrGensym switch_prefs x ->
+      st_valid st ->
+      reuse_ident x st = (y, st') ->
+      ~st_In y st.
+  Proof.
+    intros * At1 At2 Reu. unfold reuse_ident in *.
+    cases_eqn EQ; inv_equalities.
+    - intros [In|In].
+      + eapply fresh_ident_nIn; eauto.
+      + eapply At2 in In.
+        eapply st_valid_AtomOrGensym_nIn; eauto using local_not_in_switch_prefs, fresh_ident_Inids.
+    - apply PSE.mem_4 in EQ.
+      contradict EQ. destruct EQ as [In|In]; auto.
+      exfalso. eapply st_valid_AtomOrGensym_nIn; eauto using local_not_in_switch_prefs.
+  Qed.
+
+  Corollary reuse_idents_st_nIn : forall locs locs' st st',
+      Forall (AtomOrGensym switch_prefs) locs ->
+      st_valid st ->
+      mmap reuse_ident locs st = (locs', st') ->
+      Forall (fun y => ~st_In y st) locs'.
+  Proof.
+    intros * F V Map.
+    eapply mmap_values', Forall2_ignore1 in Map; eauto using reuse_ident_st_follows.
+    2:{ simpl_Forall; eauto using reuse_ident_st_valid. }
+    simpl_Forall. eapply reuse_ident_st_nIn in H4; eauto using st_follows_In.
+  Qed.
+
+  Lemma inlinelocal_block_st_nIn : forall blk Γ sub blks' locs' st st',
+      NoDupLocals Γ blk ->
+      GoodLocals switch_prefs blk ->
+      st_valid st ->
+      inlinelocal_block sub blk st = (locs', blks', st') ->
+      Forall (fun '(x, _) => ~ (st_In x st)) locs'.
+  Proof.
+    induction blk using block_ind2; intros * ND Good V IL; inv ND; inv Good;
+      repeat monadInv; try constructor.
+    - (* reset *)
+      eapply mmap2_values', Forall3_ignore13 in H0; eauto using inlinelocal_block_st_follows.
+      2:{ simpl_Forall; eauto using inlinelocal_block_st_valid. }
+      apply Forall_concat. simpl_Forall.
+      take (inlinelocal_block _ _ _ = _) and eapply H in it; eauto. simpl_Forall; eauto using st_follows_In.
+    - (* local *)
+      repeat inv_scope.
+      apply Forall_app; split.
+      + eapply Forall_forall. intros. simpl_In.
+        eapply reuse_idents_find' in H0 as (?&?&?&V1&F1&F2&Reu&Find); eauto using In_InMembers.
+        unfold rename_var. erewrite Env.union_find3'; eauto. simpl.
+        simpl_Forall. eapply reuse_ident_st_nIn in Reu; eauto.
+        contradict Reu; eauto using st_follows_In.
+      + eapply mmap2_values', Forall3_ignore13 in H3; eauto using inlinelocal_block_st_follows, reuse_idents_st_valid.
+        2:{ simpl_Forall; eauto using inlinelocal_block_st_valid. }
+        apply Forall_concat. simpl_Forall.
+        take (inlinelocal_block _ _ _ = _) and eapply H in it; eauto. simpl_Forall. contradict it.
+        eapply st_follows_In; [|eauto].
+        etransitivity; eauto. eapply mmap_st_follows; eauto. simpl_Forall; eauto using reuse_ident_st_follows.
+  Qed.
+
+  Corollary inlinelocal_blocks_st_nIn : forall blks Γ sub blks' locs' st st',
+      Forall (NoDupLocals Γ) blks ->
+      Forall (GoodLocals switch_prefs) blks ->
+      st_valid st ->
+      mmap2 (inlinelocal_block sub) blks st = (locs', blks', st') ->
+      Forall (fun '(x, _) => ~ (st_In x st)) (concat locs').
+  Proof.
+    intros * ND Good V IL.
+    eapply mmap2_values', Forall3_ignore13 in IL; eauto using inlinelocal_block_st_follows.
+    2:{ simpl_Forall; eauto using inlinelocal_block_st_valid. }
+    apply Forall_concat. simpl_Forall.
+    take (inlinelocal_block _ _ _ = _) and eapply inlinelocal_block_st_nIn in it; eauto.
+    simpl_Forall; eauto using st_follows_In.
+  Qed.
+
+  Corollary inlinelocal_block_nIn : forall blk sub xs locs' blks' st st',
+      Forall (fun x => PS.In x (used st)) xs ->
+      NoDupLocals xs blk ->
+      GoodLocals switch_prefs blk ->
+      st_valid st ->
+      inlinelocal_block sub blk st = (locs', blks', st') ->
+      Forall (fun '(x, _) => ~In x xs) locs'.
+  Proof.
+    intros * In ND Good Il V.
+    eapply inlinelocal_block_st_nIn in Il; eauto.
+    simpl_Forall. contradict Il. simpl_Forall. right; auto.
+  Qed.
+
+  Lemma mmap_inlinelocal_block_NoDupMembers : forall blks Γ sub locs' blks' st st',
+      Forall
+        (fun blk =>
+           forall Γ sub locs' blks' st st',
+             NoDupLocals Γ blk ->
+             GoodLocals switch_prefs blk ->
+             st_valid st ->
+             inlinelocal_block sub blk st = (locs', blks', st') ->
+             NoDupMembers locs') blks ->
+      Forall (NoDupLocals Γ) blks ->
+      Forall (GoodLocals switch_prefs) blks ->
+      st_valid st ->
+      mmap2 (inlinelocal_block sub) blks st = (locs', blks', st') ->
+      NoDupMembers (concat locs').
+  Proof.
+    induction blks; intros * F ND Good V IL; inv F; inv ND; inv Good;
+      repeat monadInv; simpl. constructor.
+    apply NoDupMembers_app; eauto using inlinelocal_block_st_valid.
+    - intros * In1 In2.
+      eapply inlinelocal_blocks_st_nIn in H0; eauto using inlinelocal_block_st_valid.
+      eapply inlinelocal_block_st_In in H; eauto.
+      simpl_In. simpl_Forall. contradiction.
+  Qed.
+
+  Lemma reuse_idents_rename {A} sub : forall (locs : list (ident * A)) locs' st st',
+      NoDupMembers locs ->
+      mmap reuse_ident (map fst locs) st = (locs', st') ->
+      map (rename_var (Env.union sub (Env.from_list (combine (map fst locs) locs')))) (map fst locs) = locs'.
+  Proof.
+    intros * ND Map. eapply Forall2_eq, Forall2_forall2.
+    assert (Map':=Map). eapply mmap_values, Forall2_forall2 in Map as (Len&F2).
+    rewrite map_length. split; auto.
+    intros * N Nth1 Nth2; subst.
+    erewrite map_nth' with (d':=xH); eauto.
+    unfold rename_var. erewrite Env.union_find3'; eauto. simpl; eauto.
+    apply Env.find_In_from_list. 2:now apply NoDup_NoDupMembers_combine, fst_NoDupMembers.
+    erewrite <-combine_nth; eauto. eapply nth_In.
+    now rewrite combine_length, <-Len, Nat.min_id.
+  Qed.
+
+  Lemma reuse_idents_NoDup {A} : forall (locs : list (ident * A)) locs' st st',
+      Forall (AtomOrGensym switch_prefs) (map fst locs) ->
+      st_valid st ->
+      mmap reuse_ident (map fst locs) st = (locs', st') ->
+      NoDup locs'.
+  Proof.
+    induction locs; intros * At V Reu; inv At;
+      repeat monadInv; constructor; eauto using reuse_ident_st_valid.
+    - intros In.
+      eapply reuse_ident_st_In in H as StIn.
+      eapply reuse_idents_st_nIn in H0 as StIns; eauto using reuse_ident_st_valid.
+      simpl_Forall. contradiction.
+  Qed.
+
+  Lemma inlinelocal_block_NoDupMembers : forall blk Γ sub locs' blks' st st',
+      NoDupLocals Γ blk ->
+      GoodLocals switch_prefs blk ->
+      st_valid st ->
+      inlinelocal_block sub blk st = (locs', blks', st') ->
+      NoDupMembers locs'.
+  Proof.
+    induction blk using block_ind2; intros * ND Good V IL; inv ND; inv Good;
+      repeat monadInv; try constructor.
+    - (* reset *)
+      eapply mmap_inlinelocal_block_NoDupMembers; eauto.
+    - (* local *)
+      repeat inv_scope.
+      apply NoDupMembers_app.
+      + erewrite fst_NoDupMembers, map_map, map_ext, <-map_map, reuse_idents_rename; eauto.
+        2:intros; destruct_conjs; auto.
+        eapply reuse_idents_NoDup; eauto.
+      + eapply mmap_inlinelocal_block_NoDupMembers in H3; eauto using reuse_idents_st_valid.
+      + intros * In1 In2. erewrite fst_InMembers, map_map, map_ext, <-map_map, reuse_idents_rename in In1; eauto.
+        2:intros; destruct_conjs; auto.
+        eapply inlinelocal_blocks_st_nIn in H3; eauto using reuse_idents_st_valid.
+        eapply reuse_idents_st_In in H0.
+        simpl_In. simpl_Forall. contradiction.
+  Qed.
+
+  (** *** No local block *)
+
+  Lemma inlinelocal_block_nolocal : forall blk sub locs' blks' st st',
+      noswitch_block blk ->
+      inlinelocal_block sub blk st = (locs', blks', st') ->
+      Forall nolocal_block blks'.
+  Proof.
+    induction blk using block_ind2; intros * Hns Hdl; inv Hns; repeat monadInv.
+    - (* equation *)
+      repeat constructor.
+    - (* reset *)
+      repeat constructor.
+      eapply mmap2_values, Forall3_ignore12 in H0.
+      eapply Forall_concat. simpl_Forall.
+      eapply H in H4; eauto. now simpl_Forall.
+    - (* local *)
+      eapply mmap2_values, Forall3_ignore12 in H1.
+      eapply Forall_concat. simpl_Forall.
+      eapply H in H6; eauto. now simpl_Forall.
+  Qed.
+
+  (** ** Transformation of node and program *)
+
   Program Definition inlinelocal_node (n: @node noswitch_block switch_prefs) : @node nolocal_top_block local_prefs :=
-    let res := inlinelocal_topblock (n_block n) init_st in
+    let res := inlinelocal_block (Env.empty _)
+                 (n_block n)
+                 {| fresh_st := init_st; used := PSP.of_list (map fst (n_in n ++ n_out n)) |} in
     {|
       n_name := (n_name n);
       n_hasstate := (n_hasstate n);
@@ -463,9 +971,9 @@ Module Type INLINELOCAL
       n_out := (n_out n);
       n_block := Blocal
                    (Scope
-                      (snd (fst res)++map (fun xtc => (fst xtc, ((fst (snd xtc)), snd (snd xtc), xH, None)))
-                           (st_anns (snd res)))
-                      (fst (fst res)));
+                      (map (fun xtc => (fst xtc, ((fst (snd xtc)), snd (snd xtc), xH, None)))
+                           (fst (fst res)))
+                      (snd (fst res)));
       n_ingt0 := (n_ingt0 n);
       n_outgt0 := (n_outgt0 n);
     |}.
@@ -474,61 +982,49 @@ Module Type INLINELOCAL
     pose proof (n_nodup n) as (_&Hndup).
     pose proof (n_syn n) as Hns.
     repeat esplit; eauto.
-    destruct (inlinelocal_topblock _ _) as ((?&?)&?) eqn:Hdl.
-    eapply inlinelocal_topblock_vars_perm in Hvars as (?&?&Hperm'); eauto.
+    destruct (inlinelocal_block _ _) as ((?&?)&?) eqn:Hdl.
+    eapply inlinelocal_block_vars_perm in Hvars as (?&?&Hperm'); eauto.
+    rewrite rename_vars_empty in Hperm'.
     2:{ rewrite Hperm.
         eapply NoDupLocals_incl; [|eauto]. solve_incl_app. }
     do 2 econstructor; eauto using incl_nil'. do 2 esplit; eauto.
-    unfold st_ids in *. rewrite init_st_anns, app_nil_r in Hperm'.
-    erewrite Hperm', map_app; simpl.
-    repeat apply Permutation_app_head.
-    erewrite map_map; eauto.
+    erewrite map_map, map_ext; eauto.
   Qed.
   Next Obligation.
     pose proof (n_good n) as (Hgood1&Hgood2&_).
     pose proof (n_nodup n) as (Hnd1&Hnd2).
     pose proof (n_syn n) as Hsyn.
     repeat rewrite app_nil_r.
-    destruct (inlinelocal_topblock _ _) as ((?&?)&st') eqn:Hdl. simpl.
-    split; eauto. do 2 constructor; eauto.
-    - eapply inlinelocal_topblock_NoDupLocals; eauto.
-    - specialize (st_valid_NoDup st') as Hndup.
-      apply NoDupMembers_app.
-      + eapply inlinelocal_topblock_NoDupMembers; eauto.
-      + rewrite fst_NoDupMembers, map_map; eauto.
-      + intros * Hinm1 Hinm2.
-        rewrite fst_InMembers in Hinm1, Hinm2. rewrite map_map in Hinm2.
-        eapply st_valid_AtomOrGensym_nIn in Hinm2; eauto using local_not_in_switch_prefs.
-        eapply Forall_forall; [|eapply Hinm1].
-        eapply inlinelocal_topblock_AtomOrGensym; eauto.
-    - intros ? Hinm contra. simpl_Forall.
-      apply InMembers_app in Hinm as [Hinm|Hinm].
-      + eapply inlinelocal_topblock_nIn; eauto.
-      + apply fst_InMembers in Hinm.
-        eapply st_valid_AtomOrGensym_nIn; eauto using local_not_in_switch_prefs.
-        unfold st_ids. solve_In.
+    destruct (inlinelocal_block _ _) as ((?&?)&st') eqn:Hdl. simpl.
+    split; auto. do 2 constructor; eauto.
+    - eapply inlinelocal_block_NoDupLocals; eauto.
+    - eapply inlinelocal_block_NoDupMembers in Hdl; eauto.
+      2:{ intros ? In. apply In_of_list in In. now simpl_Forall. }
+      apply NoDupMembers_map; auto.
+    - intros * In1 In2.
+      eapply inlinelocal_block_nIn in Hdl. 3-5:eauto.
+      2:{ simpl_Forall. apply In_of_list. solve_In. }
+      2:{ intros ? In. apply In_of_list in In. now simpl_Forall. }
+      simpl_In. simpl_Forall.
+      eapply Hdl. solve_In.
   Qed.
   Next Obligation.
     pose proof (n_good n) as (Hgood1&Hgood2&Hatom).
     pose proof (n_nodup n) as (Hnd1&Hnd2).
-    destruct (inlinelocal_topblock _ _) as ((?&?)&?) eqn:Hdl. simpl.
+    destruct (inlinelocal_block _ _) as ((?&?)&?) eqn:Hdl. simpl.
     pose proof (n_syn n) as Hsyn.
-    repeat split; eauto using AtomOrGensym_add.
+    repeat split; eauto using Forall_AtomOrGensym_add.
     do 2 constructor.
-    - assert (Hil:=Hdl). specialize (st_valid_prefixed f) as Hpref.
-      rewrite map_app, map_map, Forall_app; split; simpl.
-      + eapply AtomOrGensym_add, inlinelocal_topblock_AtomOrGensym; eauto.
-      + eapply Forall_impl; [|eauto]; intros; simpl in *.
-        right. do 2 eexists; eauto using PSF.add_1.
-    - eapply inlinelocal_topblock_GoodLocals; eauto.
+    - eapply inlinelocal_block_AtomOrGensym in Hdl; eauto.
+      simpl_Forall; auto.
+    - eapply inlinelocal_block_GoodLocals; eauto.
   Qed.
   Next Obligation.
     pose proof (n_syn n) as Hsyn.
-    destruct (inlinelocal_topblock _ _) as ((?&?)&?) eqn:Hdl.
+    destruct (inlinelocal_block _ _) as ((?&?)&?) eqn:Hdl.
     constructor.
-    - simpl_Forall. apply in_app_iff in H as [|]; simpl_In; auto.
-      apply inlinelocal_topblock_nolast in Hdl; auto. simpl_Forall; auto.
-    - eapply inlinelocal_topblock_nolocal; eauto.
+    - simpl_Forall. auto.
+    - eapply inlinelocal_block_nolocal; eauto.
   Qed.
 
   Global Program Instance inlinelocal_node_transform_unit: TransformUnit (@node noswitch_block switch_prefs) node :=
@@ -552,6 +1048,46 @@ Module Type INLINELOCAL
       simpl. repeat constructor.
     - destruct (find_unit f (inlinelocal_global G)) as [(?&?)|] eqn:Hfind'; simpl; try constructor.
       eapply find_unit_transform_units_backward in Hfind' as (?&?&?&?); congruence.
+  Qed.
+
+  (* Additional properties *)
+
+  Definition senv_of_anns (locs' : list (ident * ann)) : static_env :=
+    map (fun '(x, (ty, ck)) => (x, (Build_annotation ty ck xH None))) locs'.
+  Global Hint Unfold senv_of_anns : list.
+
+  Fact senv_of_anns_app : forall locs1 locs2,
+      senv_of_anns (locs1 ++ locs2) = senv_of_anns locs1 ++ senv_of_anns locs2.
+  Proof.
+    intros. apply map_app.
+  Qed.
+
+  Fact senv_of_anns_concat_incl Γ : forall locs locs',
+      In locs locs' ->
+      incl (Γ ++ senv_of_anns locs) (Γ ++ senv_of_anns (concat locs')).
+  Proof.
+    intros * In.
+    now apply incl_appr', incl_map, incl_concat.
+  Qed.
+  Global Hint Resolve senv_of_anns_concat_incl : senv.
+
+  Lemma reuse_ident_gensym : forall x y st st',
+      reuse_ident x st = (y, st') ->
+      y = x \/ exists n hint, y = gensym local hint n.
+  Proof.
+    intros * Reu.
+    unfold reuse_ident in *. cases_eqn EQ; inv_equalities.
+    - right. eapply Fresh.Ker.fresh_ident_prefixed in EQ0; eauto.
+  Qed.
+
+  Lemma reuse_idents_gensym {A} : forall (locs : list (ident * A)) locs' st st',
+      mmap reuse_ident (map fst locs) st = (locs', st') ->
+      Forall (fun x => InMembers x locs \/ exists n hint, x = gensym local hint n) locs'.
+  Proof.
+    intros * Map.
+    eapply mmap_values, Forall2_ignore1 in Map. simpl_Forall.
+    eapply reuse_ident_gensym in H1 as [|]; subst; eauto.
+    - left. now apply fst_InMembers.
   Qed.
 
 End INLINELOCAL.
