src/Lustre/InlineLocal/ILCorrectness.v
@@ -52,39 +52,19 @@ Module Type ILCORRECTNESS
     eapply Hsub, sem_var_mask in Hv; eauto. rewrite Heq; eauto.
   Qed.
 
-  Import Fresh Facts Tactics.
   Import List.
 
-  Fact find_pred_snd_nNone : forall (sub: Env.t ident) x y,
-      Env.find x sub = Some y ->
-      Env.find_pred (fun _ y' => Var y' ==b Var y) sub <> None.
+  Fact find_snd_spec {A} : forall (locs : list (ident * A)) (locs' : list ident) x y,
+      NoDup locs' ->
+      In (x, y) (combine (map fst locs) locs') ->
+      find (fun '(_, y') => Var y' ==b Var y) (combine (map fst locs) locs') = Some (x, y).
   Proof.
-    unfold Env.find_pred. intros *.
-    apply Env.Props.P.fold_rec.
-    - intros * Hempty Hfind.
-      apply Hempty in Hfind as [].
-    - intros * _ _ Hadd Hrec Hfind.
-      unfold Env.Props.P.Add in Hadd. rewrite Hadd in Hfind.
-      destruct (ident_eq_dec x k); subst.
-      * rewrite Env.gss in Hfind. inv Hfind.
-        rewrite equiv_decb_refl. congruence.
-      * rewrite Env.gso in Hfind; auto.
-        destruct (_ ==b _); auto. congruence.
-  Qed.
-
-  Fact find_pred_snd_spec : forall (sub: Env.t ident) x y,
-      NoDup (map snd (Env.elements sub)) ->
-      Env.find x sub = Some y ->
-      Env.find_pred (fun _ y' => Var y' ==b Var y) sub = Some (x, y).
-  Proof.
-    intros * Hnd Hfind.
-    destruct (Env.find_pred _ _) as [(?&?)|] eqn:Hfind'.
-    - apply Env.find_pred_spec in Hfind' as (Hfind'&Heq).
-      rewrite equiv_decb_equiv in Heq; inv Heq.
-      eapply Env.NoDup_snd_elements in Hfind; eauto; subst.
-      reflexivity.
-    - exfalso.
-      eapply find_pred_snd_nNone; eauto.
+    induction locs; intros * Nd In; simpl in *; [inv In|].
+    inv Nd; [inv In|]. inv In; inv_equalities.
+    - now rewrite equiv_decb_refl.
+    - cases_eqn Eq.
+      rewrite equiv_decb_equiv in Eq; inv Eq.
+      eapply in_combine_r in H1. contradiction.
   Qed.
 
   Section inlinelocal_node_sem.
@@ -145,73 +125,123 @@ Module Type ILCORRECTNESS
     Local Hint Resolve <- fst_InMembers InMembers_idck InMembers_idty : datatypes.
     Local Hint Resolve -> fst_InMembers InMembers_idck InMembers_idty : datatypes.
 
-    Definition st_senv (st: fresh_st local _) := senv_of_tyck (st_anns st).
-
-    Fact mmap_inlinelocal_block_sem : forall Γ blks sub Γ' blks' st st' bs Hi1 Hi2,
+    Fact mmap_inlinelocal_block_sem : forall Γ blks sub Γ' Γ'' locs' blks' st st' bs Hi1 Hi2,
         Forall
-          (fun blk => forall sub Γ' blks' st st' bs Hi1 Hi2,
-               (forall x, ~IsLast (Γ++Γ') x) ->
+          (fun blk => forall sub Γ' Γ'' locs' blks' st st' bs Hi1 Hi2,
+               (forall x, ~IsLast (Γ++Γ'++Γ'') x) ->
                (forall x, IsVar Γ x -> ~IsVar Γ' x) ->
                (forall x, Env.In x sub <-> IsVar Γ' x) ->
+               (forall x y, Env.MapsTo x y sub -> InMembers y Γ' \/ exists n hint, y = gensym local hint n) ->
                (forall x y vs, Env.find x sub = Some y -> sem_var Hi1 (Var x) vs -> sem_var Hi2 (Var y) vs) ->
                (forall x vs, IsVar Γ x -> sem_var Hi1 (Var x) vs -> sem_var Hi2 (Var x) vs) ->
-               (forall x y, Env.MapsTo x y sub -> exists n : ident, y = gensym local (Some x) n) ->
                NoDupMembers (Γ++Γ') ->
                noswitch_block blk ->
-               NoDupLocals (map fst (Γ++Γ')) blk ->
+               NoDupLocals (map fst Γ++map fst Γ'++map fst Γ'') blk ->
                Forall (AtomOrGensym switch_prefs) (map fst Γ) ->
                GoodLocals switch_prefs blk ->
-               wc_env (idck (Γ++Γ')) ->
-               wc_block G1 (Γ++Γ') blk ->
                dom_ub Hi1 (Γ++Γ') ->
                sem_block_ck G1 Hi1 bs blk ->
-               dom Hi2 (Γ++st_senv st) ->
-               sc_vars (Γ++st_senv st) Hi2 bs ->
-               inlinelocal_block sub blk st = (blks', st') ->
+               dom Hi2 (Γ++Γ'') ->
+               sc_vars (Γ++Γ'') Hi2 bs ->
+               st_valid st ->
+               Forall (fun x => st_In x st) (map fst (Γ ++ Γ'')) ->
+               inlinelocal_block sub blk st = (locs', blks', st') ->
                exists Hi3,
                  Hi2 ⊑ Hi3 /\
-                 dom Hi3 (Γ++st_senv st') /\
-                 sc_vars (Γ++st_senv st') Hi3 bs /\
+                 dom Hi3 (Γ++Γ''++senv_of_anns locs') /\
+                 sc_vars (Γ++Γ''++senv_of_anns locs') Hi3 bs /\
                  Forall (sem_block_ck G2 Hi3 bs) blks')
           blks ->
-        (forall x, ~IsLast (Γ++Γ') x) ->
+        (forall x, ~IsLast (Γ++Γ'++Γ'') x) ->
         (forall x, IsVar Γ x -> ~IsVar Γ' x) ->
         (forall x, Env.In x sub <-> IsVar Γ' x) ->
+        (forall x y, Env.MapsTo x y sub -> InMembers y Γ' \/ exists n hint, y = gensym local hint n) ->
         (forall x y vs, Env.find x sub = Some y -> sem_var Hi1 (Var x) vs -> sem_var Hi2 (Var y) vs) ->
         (forall x vs, IsVar Γ x -> sem_var Hi1 (Var x) vs -> sem_var Hi2 (Var x) vs) ->
-        (forall x y, Env.MapsTo x y sub -> exists n : ident, y = gensym local (Some x) n) ->
         NoDupMembers (Γ++Γ') ->
         Forall noswitch_block blks ->
-        Forall (NoDupLocals (map fst (Γ++Γ'))) blks ->
+        Forall (NoDupLocals (map fst Γ++map fst Γ'++map fst Γ'')) blks ->
         Forall (AtomOrGensym switch_prefs) (map fst Γ) ->
         Forall (GoodLocals switch_prefs) blks ->
-        wc_env (idck (Γ++Γ')) ->
-        Forall (wc_block G1 (Γ++Γ')) blks ->
         dom_ub Hi1 (Γ++Γ') ->
         Forall (sem_block_ck G1 Hi1 bs) blks ->
-        dom Hi2 (Γ++st_senv st) ->
-        sc_vars (Γ++st_senv st) Hi2 bs ->
-        mmap (inlinelocal_block sub) blks st = (blks', st') ->
+        dom Hi2 (Γ++Γ'') ->
+        sc_vars (Γ++Γ'') Hi2 bs ->
+        st_valid st ->
+        Forall (fun x => st_In x st) (map fst (Γ ++ Γ'')) ->
+        mmap2 (inlinelocal_block sub) blks st = (locs', blks', st') ->
         exists Hi3,
           Hi2 ⊑ Hi3 /\
-          dom Hi3 (Γ++st_senv st') /\
-          sc_vars (Γ++st_senv st') Hi3 bs /\
+          dom Hi3 (Γ++Γ''++senv_of_anns (concat locs')) /\
+          sc_vars (Γ++Γ''++senv_of_anns (concat locs')) Hi3 bs /\
           Forall (sem_block_ck G2 Hi3 bs) (concat blks').
     Proof with eauto.
       induction blks;
-        intros * Hf Hnl Hdisj Hsubin Hsub Hnsub Hsubgensym Hnd1 Hns Hnd2 Hatgen Hgood Hwenv Hwc Hub Hsem Hdom Hsc Hmmap;
-        inv Hf; inv Hns; inv Hnd2; inv Hgood; inv Hwc; inv Hsem; repeat inv_bind; simpl in *.
-      - exists Hi2. repeat (split; auto with env). reflexivity.
-      - assert (Hdl:=H).
-        eapply H1 with (Hi1:=Hi1) (Hi2:=Hi2)
-          in H as (Hi3&Href1&Hdom1&Hsc1&Hsem1)... clear H1.
-        eapply IHblks with (Hi1:=Hi1) (Hi2:=Hi3)
-          in H0 as (Hi4&Href3&Hdom3&Hsc3&Hsem3)... clear IHblks H2.
-        2,3:intros; eauto using sem_var_refines.
-        exists Hi4. repeat (split; auto).
-        + etransitivity...
-        + apply Forall_app; split; auto.
-          eapply Forall_impl; [|eauto]; intros; eauto using sem_block_refines.
+        intros * Hf Hnl Hdisj Hsubin Hsubgen Hsub Hnsub Hnd1 Hns Hnd2 Hatgen Hgood Hub Hsem Hdom Hsc V InSt Hmmap;
+        inv Hf; inv Hns; inv Hnd2; inv Hgood; (* inv Hwc; *) inv Hsem; repeat monadInv; simpl in *.
+      - repeat rewrite app_nil_r. exists Hi2. repeat (split; auto with env). reflexivity.
+      - assert (Il:=H). assert (Ils:=H0).
+        eapply H1 with (Hi1:=Hi1) (Hi2:=Hi2) in H as (Hi3&Href3&Hdom3&Hsc3&Hsem3); eauto.
+        eapply IHblks with (Hi1:=Hi1) (Hi2:=Hi2) in H0 as (Hi4&Href4&Hdom4&Hsc4&Hsem4);
+          eauto using inlinelocal_block_st_valid.
+        2:{ simpl_Forall. eapply inlinelocal_block_st_follows in Il; eauto using st_follows_In. }
+        clear H1 IHblks H2.
+        remember (FEnv.union Hi3 Hi4) as Hi5.
+        assert (FEnv.refines (@EqSt _) Hi4 Hi5) as Ref2.
+        { subst. eapply FEnv.union_refines4'; eauto using EqStrel_Reflexive. }
+        assert (FEnv.refines (@EqSt _) Hi3 Hi5) as Ref1.
+        { subst. intros [] ? Find.
+          2:{ exfalso. apply FEnv.find_In, Hdom3 in Find as In.
+              rewrite app_assoc, IsLast_app in In. destruct In as [In|In].
+              - eapply Hnl. repeat rewrite IsLast_app in *. destruct In; eauto.
+              - inv In. simpl_In. congruence. }
+          apply FEnv.find_In in Find as In. apply Hdom3 in In.
+          rewrite app_assoc, IsVar_app in In. destruct In as [In|In].
+          - assert (sem_var Hi2 (Var x4) v) as Var. 2:inversion_clear Var as [???? Find' Eq].
+            { eapply sem_var_refines' in Href3; eauto.
+              - now apply Hdom.
+              - econstructor; eauto. reflexivity. }
+            eapply Href4 in Find' as (?&Eq2&Find').
+            eapply Ref2 in Find' as (?&Eq3&Find'').
+            do 2 esplit; [|eauto]. now rewrite Eq, Eq2, Eq3.
+          - erewrite FEnv.union2; eauto. do 2 esplit; eauto. reflexivity.
+            apply FEnv.not_find_In. intros In2. eapply Hdom4 in In2.
+            rewrite app_assoc, IsVar_app in In2. destruct In2 as [In2|In2].
+            + eapply inlinelocal_block_st_nIn in Il; eauto.
+              clear - InSt In In2 Il. inv In. inv In2. simpl_In. simpl_Forall. contradiction.
+            + eapply inlinelocal_blocks_st_nIn in Ils; eauto using inlinelocal_block_st_valid.
+              eapply inlinelocal_block_st_In in Il; [|eauto].
+              clear - In In2 Ils Il. inv In. inv In2. simpl_In. simpl_Forall. contradiction.
+        }
+        exists Hi5; subst. split; [|split; [|split; [|apply Forall_app; split]]].
+        + etransitivity; eauto.
+        + rewrite senv_of_anns_app. unfold dom.
+          destruct Hdom3 as (D3&DL3). destruct Hdom4 as (D4&DL4).
+          split; intros ?; rewrite FEnv.union_In; [rewrite D3, D4|rewrite DL3, DL4];
+            repeat rewrite IsVar_app; repeat rewrite IsLast_app;
+            split; intros; repeat take (_ \/ _) and destruct it; auto.
+        + rewrite senv_of_anns_app.
+          split.
+          2:{ intros * _ L. exfalso.
+              rewrite app_assoc, IsLast_app, IsLast_app with (env1:=senv_of_anns _) in L.
+              destruct L as [L|[L|L]].
+              2,3:clear - L; inv L; simpl_In; congruence.
+              eapply Hnl. repeat rewrite IsLast_app in *. destruct L; eauto. }
+          intros * Ck Var.
+          rewrite app_assoc, HasClock_app, HasClock_app with (env1:=senv_of_anns _) in Ck. destruct Ck as [Ck|[Ck|Ck]].
+          * destruct Hsc as (Sc&_). eapply sem_clock_refines, Sc; eauto. eapply var_history_refines; etransitivity; eauto.
+            eapply sem_var_refines'; [| |eauto]. 2:etransitivity; eauto.
+            eapply Hdom; eauto with senv.
+          * destruct Hsc3 as (Sc&_). eapply sem_clock_refines, Sc; eauto using var_history_refines.
+            repeat rewrite HasClock_app; eauto.
+            eapply sem_var_refines'; [|eauto|eauto].
+            eapply Hdom3. repeat rewrite IsVar_app; eauto with senv.
+          * destruct Hsc4 as (Sc&_). eapply sem_clock_refines, Sc; eauto using var_history_refines.
+            repeat rewrite HasClock_app; eauto.
+            eapply sem_var_refines'; [|eauto|eauto].
+            eapply Hdom4. repeat rewrite IsVar_app; eauto with senv.
+        + simpl_Forall. eauto using sem_block_refines.
+        + simpl_Forall. eauto using sem_block_refines.
     Qed.
 
     Ltac inv_scope :=
@@ -224,41 +254,43 @@ Module Type ILCORRECTNESS
        - Hi2 : history after renaming of the enclosing blocks
        - Hi3 : refines Hi2 by adding the renamed variables of the subblocks
      *)
-    Lemma inlinelocal_block_sem Γ : forall blk sub Γ' blks' st st' bs Hi1 Hi2,
-        (forall x, ~IsLast (Γ++Γ') x) ->
+    Lemma inlinelocal_block_sem Γ : forall blk sub Γ' Γ'' locs' blks' st st' bs Hi1 Hi2,
+        (forall x, ~IsLast (Γ++Γ'++Γ'') x) ->
         (forall x, IsVar Γ x -> ~IsVar Γ' x) ->
         (forall x, Env.In x sub <-> IsVar Γ' x) ->
+        (forall x y, Env.MapsTo x y sub -> InMembers y Γ' \/ exists n hint, y = gensym local hint n) ->
         (forall x y vs, Env.find x sub = Some y -> sem_var Hi1 (Var x) vs -> sem_var Hi2 (Var y) vs) ->
         (forall x vs, IsVar Γ x -> sem_var Hi1 (Var x) vs -> sem_var Hi2 (Var x) vs) ->
-        (forall x y, Env.MapsTo x y sub -> exists n, y = gensym local (Some x) n) ->
         NoDupMembers (Γ++Γ') ->
         noswitch_block blk ->
-        NoDupLocals (map fst (Γ++Γ')) blk ->
+        NoDupLocals (map fst Γ++map fst Γ'++map fst Γ'') blk ->
         Forall (AtomOrGensym switch_prefs) (map fst Γ) ->
         GoodLocals switch_prefs blk ->
-        wc_env (idck (Γ++Γ')) ->
-        wc_block G1 (Γ++Γ') blk ->
         dom_ub Hi1 (Γ++Γ') ->
         sem_block_ck G1 Hi1 bs blk ->
-        dom Hi2 (Γ ++ st_senv st) ->
-        sc_vars (Γ++st_senv st) Hi2 bs ->
-        inlinelocal_block sub blk st = (blks', st') ->
+        dom Hi2 (Γ ++ Γ'') ->
+        sc_vars (Γ++Γ'') Hi2 bs ->
+        st_valid st ->
+        Forall (fun x => st_In x st) (map fst (Γ ++ Γ'')) ->
+        inlinelocal_block sub blk st = (locs', blks', st') ->
         exists Hi3,
           Hi2 ⊑ Hi3 /\
-          dom Hi3 (Γ++st_senv st') /\
-          sc_vars (Γ++st_senv st') Hi3 bs /\
+          dom Hi3 (Γ++Γ''++senv_of_anns locs') /\
+          sc_vars (Γ++Γ''++senv_of_anns locs') Hi3 bs /\
           Forall (sem_block_ck G2 Hi3 bs) blks'.
     Proof with eauto with datatypes.
       induction blk using block_ind2;
-        intros * Hnl Hdisj Hsubin Hsub Hnsub Hsubgensym Hnd1 Hns Hnd2 Hgenat Hgood Hwenv Hwc Hub Hsem Hdom Hsc Hdl;
-        inv Hns; inv Hnd2; inv Hgood; inv Hwc; inv Hsem; repeat inv_bind; simpl.
+        intros * Hnl Hdisj Hsubin Hsubgen Hsub Hnsub Hnd1 Hns Hnd2 Hgenat Hgood Hub Hsem Hdom Hsc V StIn Hdl;
+        inv Hns; inv Hnd2; inv Hgood; inv Hsem; repeat monadInv; simpl.
 
       - (* equation *)
+        repeat rewrite app_nil_r.
         exists Hi2. repeat (split; auto with env). reflexivity.
-        constructor; auto. constructor.
+        repeat constructor; auto.
         eapply subclock_equation_sem with (H:=Hi1); eauto using sem_ref_sem_equation.
         + constructor; reflexivity.
-        + intros * Hl. exfalso. apply sem_var_In, Hub in Hl. eapply Hnl; eauto.
+        + intros * Hl. exfalso. apply sem_var_In, Hub in Hl.
+          eapply Hnl. repeat rewrite IsLast_app in *. destruct Hl; eauto.
         + intros * Hnone Hv.
           assert (Hin:=Hv). eapply sem_var_In, Hub in Hin.
           repeat rewrite map_app, in_app_iff in Hin.
@@ -266,13 +298,13 @@ Module Type ILCORRECTNESS
           * exfalso. eapply Env.Props.P.F.not_find_in_iff in Hnone. eapply Hnone, Hsubin...
 
       - (* reset *)
-        rename x into blks'.
+        rename x into locs', x0 into blks'.
         assert (forall k, exists Hi4, (CStr.mask_hist k r Hi2) ⊑ (CStr.mask_hist k r Hi4) /\
-                            dom (CStr.mask_hist k r Hi4) (Γ++st_senv st') /\
-                            sc_vars (Γ++st_senv st') (mask_hist k r Hi4) (maskb k r bs) /\
+                            dom (CStr.mask_hist k r Hi4) (Γ++Γ''++senv_of_anns (concat locs')) /\
+                            sc_vars (Γ++Γ''++senv_of_anns (concat locs')) (mask_hist k r Hi4) (maskb k r bs) /\
                             Forall (sem_block_ck G2 (mask_hist k r Hi4) (maskb k r bs)) (concat blks')) as Hblks.
-        { intros k. specialize (H13 k).
-          eapply mmap_inlinelocal_block_sem with (Hi2:=CStr.mask_hist k r Hi2) in H13
+        { intros k. specialize (H10 k).
+          eapply mmap_inlinelocal_block_sem with (Hi2:=CStr.mask_hist k r Hi2) in H10
             as (Hi4&Href1&Hdom1&Hsc1&Hsem1); eauto.
           2:{ intros ??? Hfind Hv.
               eapply sem_var_mask_inv in Hv as (?&Hv&Hmask).
@@ -284,30 +316,29 @@ Module Type ILCORRECTNESS
           2:{ eapply dom_map; eauto. }
           2:{ eapply sc_vars_mask in Hsc; eauto; subst. }
           assert (FEnv.Equiv (@EqSt _) Hi4 (CStr.mask_hist k r Hi4)) as Heqmask.
-          { unfold st_ids in Hdom1.
-            eapply slower_mask_hist. eapply sc_vars_slower_hist in Hsc1; eauto.
+          { eapply slower_mask_hist. eapply sc_vars_slower_hist in Hsc1; eauto.
             simpl_app. auto using dom_dom_ub.
           }
           exists Hi4. split; [|split; [|split]].
           + rewrite <-Heqmask; auto.
           + apply dom_map; auto.
           + unfold mask_hist. simpl. eapply sc_vars_morph. 1,3,4:eauto; reflexivity. auto.
-          + eapply Forall_impl; [|eauto]; intros. unfold mask_hist.
+          + simpl_Forall. unfold mask_hist.
             eapply sem_block_ck_morph; eauto. reflexivity.
         }
         unfold mask_hist.
         eapply consolidate_mask_hist
           with (P := fun k H'k =>
                        (CStr.mask_hist k r Hi2) ⊑ H'k /\
-                       dom H'k (Γ++st_senv st') /\
-                       sc_vars (Γ++st_senv st') H'k (maskb k r bs) /\
+                       dom H'k (Γ++Γ''++senv_of_anns (concat locs')) /\
+                       sc_vars (Γ++Γ''++senv_of_anns (concat locs')) H'k (maskb k r bs) /\
                        Forall (sem_block_ck G2 H'k (maskb k r bs)) (concat blks'))
         in Hblks as (Hi4&HHi4).
-        2:{ intros ????? Heq (?&?&(?&?)&?); subst. split; [|split; [|repeat split]].
+        2:{ intros ????? Heq (Ref&Dom&(Sc1&Sc2)&Sem); subst. split; [|split; [|repeat split]].
             - rewrite <-Heq; auto.
-            - split; intros ?; rewrite <-Heq; apply H10.
-            - intros. rewrite <-Heq. eapply H11; eauto. now rewrite Heq.
-            - intros. rewrite <-Heq. eapply H14; eauto. now rewrite Heq.
+            - split; intros ?; rewrite <-Heq; apply Dom.
+            - intros. rewrite <-Heq. eapply Sc1; eauto. now rewrite Heq.
+            - intros. rewrite <-Heq. eapply Sc2; eauto. now rewrite Heq.
             - simpl_Forall.
               eapply sem_block_ck_morph; eauto. reflexivity.
         }
@@ -322,7 +353,8 @@ Module Type ILCORRECTNESS
           * eapply sem_exp_refines; [eauto|].
             eapply subclock_exp_sem with (H:=Hi1); eauto using sem_ref_sem_exp.
             1:{ constructor; reflexivity. }
-            { intros * Hl. apply sem_var_In, Hub in Hl. exfalso; eapply Hnl; eauto. }
+            { intros * Hl. apply sem_var_In, Hub in Hl. exfalso.
+              eapply Hnl. repeat rewrite IsLast_app in *. destruct Hl; eauto. }
             { intros * Hnone Hv.
               assert (Hin:=Hv). eapply sem_var_In, Hub in Hin; eauto.
               repeat rewrite map_app, in_app_iff in Hin.
@@ -333,159 +365,156 @@ Module Type ILCORRECTNESS
 
       - (* local *)
         repeat inv_scope.
-        assert (forall x, Env.In x x0 <-> InMembers x locs) as Hsubin'.
-        { intros. split; intros * Hin.
-          - eapply fresh_idents_rename_sub1 in Hin; [|eauto].
-            unfold idty in *. erewrite fst_InMembers, map_map, map_ext, <-fst_InMembers in Hin...
-            intros; destruct_conjs...
-          - eapply fresh_idents_rename_sub2 in H0.
-            unfold idty in *. erewrite fst_InMembers, map_map, map_ext, <-fst_InMembers in H0...
-            2:intros; destruct_conjs; auto.
-            apply H0 in Hin as (?&?&?&_); eauto. econstructor...
-        }
-        assert (forall x, FEnv.In x Hi2 ->
-                     ~FEnv.In x (fun x => obind (Env.find_pred (fun _ y => Var y ==b x) x0) (fun '(x, _) => Hi' (Var x)))) as Hdisj2.
-        { intros ? Hin2 (?&Hfind1).
-          destruct x3.
-          2:{ apply Hdom, IsLast_app in Hin2 as [Hin2|Hin2]. 2:inv Hin2; simpl_In; congruence.
-              eapply Hnl, IsLast_app; eauto. }
-          apply obind_inversion in Hfind1 as ((?&?)&Hfind1&Hfind2).
-          apply Env.find_pred_spec in Hfind1 as (Hfind1&Heq). rewrite equiv_decb_equiv in Heq; inv Heq.
-          assert (Hfind1':=Hfind1). eapply fresh_idents_rename_sub_gensym in Hfind1' as (?&?); eauto; subst.
-          apply Hdom, IsVar_app in Hin2 as [Hin2|Hin2]; inv Hin2; simpl_In.
-          - simpl_Forall.
-            eapply contradict_AtomOrGensym in Hgenat; eauto using local_not_in_switch_prefs.
-          - eapply fresh_idents_rename_sub_nIn in H0; eauto. eapply H0; solve_In.
-        }
-        assert (forall x, Env.In x sub -> ~Env.In x x0) as Hsub1.
-        { intros ?. rewrite Hsubin, Hsubin'. intros Hin1 Hin2.
-          eapply H13... inv Hin1; simpl_In; do 2 esplit; eauto with datatypes. auto. }
-        assert (NoDup (map snd (Env.elements x0))) as Hnd2.
-        {  eapply fresh_idents_rename_sub_NoDup in H0; eauto.
-           apply NoDupMembers_map; auto. intros; destruct_conjs; auto. }
-        assert (Forall nolocal_block (concat x2)) as Hnlo.
-        { apply Forall_concat.
-          apply mmap_values, Forall2_ignore1 in H5. simpl_Forall.
-          apply inlinelocal_block_nolocal in H5; auto; simpl_Forall; auto. }
-        assert (Hi2 ⊑ Hi2 + (fun x3 => obind (Env.find_pred (fun (_ : Env.key) (y : ident) => Var y ==b x3) x0) (fun '(x4, _) => Hi' (Var x4)))) as Href.
+        take (forall x, InMembers x locs -> ~_) and rename it into Hnd'; eauto.
+
+        assert (forall y, Env.In y (Env.from_list (combine (map fst locs) x)) <-> InMembers y locs) as Hsubin'.
+        { intros.
+          rewrite Env.In_from_list, <-In_InMembers_combine, fst_InMembers; try reflexivity.
+          now apply mmap_values, Forall2_length in H0. }
+
+        remember (fun y => obind (List.find (fun '(_, y') => Var y' ==b y) (combine (map fst locs) x)) (fun '(x, _) => Hi' (Var x))) as Hi2'.
+
+        assert (forall y, FEnv.In (Var y) Hi2 -> ~In y x) as Hdisj2.
+        { subst. intros * In1 In2. eapply Hdom in In1. inv In1. simpl_In.
+          eapply reuse_idents_st_nIn in H0; eauto. simpl_Forall.
+          contradiction. }
+
+        assert (forall x, FEnv.In x Hi2 -> ~FEnv.In x Hi2') as Hdisj2'.
+        { subst. intros * In1 (?&Find2).
+          apply obind_inversion in Find2 as ((?&?)&F1&F2).
+          apply find_some in F1 as (In&Eq). rewrite equiv_decb_equiv in Eq; inv Eq.
+          eapply Hdisj2; eauto using in_combine_r. }
+
+        assert (forall y, Env.In y sub -> ~Env.In y (Env.from_list (combine (map fst locs) x))) as Hsub1.
+        { intros ?. rewrite Hsubin, Hsubin'. intros In1 In2.
+          eapply Hnd'; eauto. clear - In1. rewrite 2 in_app_iff. right; left. inv In1. solve_In. }
+        assert (forall x1 x2, Env.MapsTo x1 x2 sub -> ~ Env.In x2 (Env.from_list (combine (map fst locs) x))) as Hsub2.
+        { intros ??. rewrite Hsubin'. intros Hin1 Hin2.
+          eapply Hsubgen in Hin1 as [Hin|(?&?&Hgen)]; subst.
+          - eapply Hnd'; eauto. rewrite 2 in_app_iff; eauto with datatypes.
+          - simpl_In. simpl_Forall.
+            eapply Fresh.Facts.contradict_AtomOrGensym; eauto using local_not_in_switch_prefs. }
+
+        assert (Hi2 ⊑ Hi2 + Hi2') as Ref.
         { intros ?? Hfind. do 2 esplit; try reflexivity.
           apply FEnv.union2; auto.
-          destruct (obind _ _) eqn:Hb; auto. apply obind_inversion in Hb; destruct_conjs.
-          exfalso.
-          eapply Hdisj2. 1,2:econstructor; eauto. rewrite H1; eauto. }
+          eapply FEnv.not_find_In, Hdisj2'. econstructor; eauto. }
+
+        assert (dom Hi2' (senv_of_anns (map (fun '(x3, (ty, ck, _, _)) => (rename_var (Env.union sub (Env.from_list (combine (map fst locs) x))) x3, (ty, rename_in_clock (Env.union sub (Env.from_list (combine (map fst locs) x))) ck))) locs))) as Hdom'.
+        { subst; split.
+          - intros ?. unfold senv_of_anns. erewrite IsVar_fst, 2 map_map.
+            split; intros In.
+            + inv In. apply obind_inversion in H1 as ((?&?)&Find&Find').
+              apply find_some in Find as (In&Eq).
+              rewrite equiv_decb_equiv in Eq. inv Eq.
+              eapply in_combine_l in In as InL. solve_In.
+              unfold rename_var. erewrite Env.union_find3'; [|eapply Env.find_In_from_list]; eauto. auto.
+              now apply NoDup_NoDupMembers_combine, fst_NoDupMembers.
+            + simpl_In.
+              assert (FEnv.In (Var i) Hi') as [? Find] by (eapply H6; econstructor; solve_In).
+              econstructor. erewrite find_snd_spec; simpl; eauto using reuse_idents_NoDup.
+              assert (length (map fst locs) = length x) as EqLen by now apply mmap_values, Forall2_length in H0.
+              assert (exists y, In (i, y) (combine (map fst locs) x)) as (?&In).
+              { eapply in_map with (f:=fst), In_nth with (d:=xH) in Hin as (?&Len&Nth). simpl in *.
+                esplit. erewrite <-Nth, <-combine_nth with (y:=xH); eauto. eapply nth_In.
+                rewrite combine_length, <-EqLen, Nat.min_id; auto. }
+              unfold rename_var. erewrite Env.union_find3'; [|eapply Env.find_In_from_list]; eauto. auto.
+              now apply NoDup_NoDupMembers_combine, fst_NoDupMembers.
+          - split; intros In; exfalso; [|inv In; simpl_In; congruence].
+            inv In. apply obind_inversion in H1 as ((?&?)&Find&_).
+            apply find_some in Find as (_&Eq).
+            rewrite equiv_decb_equiv in Eq. inv Eq.
+        }
+
         eapply mmap_inlinelocal_block_sem with
-            (Γ':=Γ'++senv_of_locs locs) (Hi1:=Hi1 + Hi') (Hi2:=Hi2 + fun x => obind (Env.find_pred (fun _ y => Var y ==b x) x0) (fun '(x, _) => Hi' (Var x)))
-            (sub:=Env.union sub x0) (st:=x1)
-          in H5 as (Hi3&Href1&Hdom1&(Hsc11&Hsc12)&Hsem1); eauto. clear H.
-        + exists Hi3. repeat (split; eauto).
-          etransitivity...
-        + rewrite app_assoc, NoLast_app; split; auto.
-          intros * Hla; inv Hla; simpl_In; simpl_Forall. subst; simpl in *; congruence.
+            (Γ':=Γ'++senv_of_locs locs) (Hi1:=Hi1 + Hi') (Hi2:=Hi2 + Hi2') in H5 as (Hi3&Href1&Hdom1&Hsc1&Hsem1); eauto; clear H.
+        + exists Hi3. split; [|split; [|split]]; eauto.
+          * etransitivity...
+          * rewrite senv_of_anns_app, app_assoc with (n:=senv_of_anns _); eauto.
+          * rewrite senv_of_anns_app, app_assoc with (n:=senv_of_anns _); eauto.
+        + rewrite app_assoc. repeat rewrite NoLast_app in *. destruct_conjs.
+          repeat split; auto.
+          * intros * L. inv L. simpl_In. simpl_Forall. subst; simpl in *; congruence.
+          * intros * L. inv L. simpl_In. congruence.
         + intros ?. rewrite IsVar_app. intros Hinm1 [Hinm2|Hinm2].
           * eapply Hdisj; eauto.
-          * apply IsVar_senv_of_locs in Hinm2. take (forall x, InMembers x locs -> ~_) and eapply it...
-            rewrite <-IsVar_fst, IsVar_app; auto.
+          * apply IsVar_senv_of_locs in Hinm2. eapply Hnd'; eauto.
+            rewrite 2 in_app_iff, <-IsVar_fst; auto.
         + intros ?. rewrite Env.union_In, Hsubin, Hsubin', IsVar_app, IsVar_senv_of_locs.
-          split; intros [?|?]...
+          reflexivity.
+        + intros ?? Hfind. rewrite InMembers_app, InMembers_senv_of_locs.
+         eapply Env.union_find4 in Hfind as [Hfind|Hfind]; eauto.
+         * eapply Hsubgen in Hfind as [|]; eauto.
+         * eapply Env.from_list_find_In, in_combine_r in Hfind.
+           eapply reuse_idents_gensym in H0. simpl_Forall. destruct H0; eauto.
         + intros ??? Hfind Hv.
           erewrite sem_var_disj_union; eauto.
           eapply Env.union_find4 in Hfind as [Hfind|Hfind]; eapply sem_var_union in Hv as [Hv|Hv]; eauto.
           * exfalso. apply Env.find_In, Hsubin in Hfind.
             apply sem_var_In, H6, IsVar_senv_of_locs in Hv.
             take (forall x, InMembers x locs -> ~_) and eapply it...
-            rewrite <-IsVar_fst, IsVar_app; auto.
+            rewrite 2 in_app_iff, <-2 IsVar_fst; auto.
           * exfalso. apply Env.find_In, Hsubin' in Hfind.
             apply sem_var_In, Hub in Hv.
             take (forall x, InMembers x locs -> ~_) and eapply it...
-            rewrite <-IsVar_fst; auto.
+            rewrite app_assoc, in_app_iff. left. rewrite <-map_app, <-IsVar_fst; auto.
           * right. inv Hv. econstructor; eauto.
-            erewrite find_pred_snd_spec; eauto.
+            apply Env.from_list_find_In in Hfind.
+            erewrite find_snd_spec; eauto using reuse_idents_NoDup.
         + intros ?? Hfind Hv.
           erewrite sem_var_disj_union; eauto.
           eapply sem_var_union in Hv as [Hv|Hv]; eauto.
           exfalso. apply sem_var_In, H6, IsVar_senv_of_locs in Hv.
-          take (forall x, InMembers x locs -> ~_) and eapply it...
-          rewrite <-IsVar_fst, IsVar_app; auto.
-        + intros ?? Hfind.
-          eapply Env.union_find4 in Hfind as [Hfind|Hfind]...
-          eapply fresh_idents_rename_sub_gensym...
-        + rewrite app_assoc.
-          eapply NoDupMembers_app; eauto.
-          * rewrite NoDupMembers_senv_of_locs; auto.
-          * intros ? Hinm Hinm2. rewrite InMembers_senv_of_locs in Hinm2.
-            take (forall x, InMembers x locs -> ~_) and eapply it...
-        + rewrite app_assoc, map_app, map_fst_senv_of_locs; auto.
-        + unfold wc_env in *. simpl_app. rewrite app_assoc, Forall_app; split; simpl_Forall.
-          * eapply wc_clock_incl; [|eauto]. solve_incl_app.
-          * simpl_app; auto.
-        + rewrite app_assoc; auto.
-        + eapply local_hist_dom_ub in H6; eauto. now rewrite app_assoc.
-        + destruct Hdom as (Dom&DomL).
-          eapply fresh_idents_rename_ids in H0 as ?; subst; eauto. 2:apply NoDupMembers_map; auto; intros; destruct_conjs; auto.
-          split; intros ?; unfold st_senv, senv_of_tyck; erewrite FEnv.union_In, fresh_idents_rename_anns; eauto.
-          1,2:erewrite map_app, (Permutation_app_comm (map _ _)), app_assoc.
-          1:rewrite IsVar_app, Dom. 2:rewrite IsLast_app, DomL.
-          1,2:apply or_iff_compat_l; split; intros In.
-          * destruct In as (?&Find). apply obind_inversion in Find as ((?&?)&Find&?).
-            apply Env.find_pred_spec in Find as (Find&Eq). rewrite equiv_decb_equiv in Eq. inv Eq.
-            eapply fresh_idents_rename_sub1 in H0; [|econstructor; eauto].
-            clear - Find H0. econstructor. solve_In.
-            now rewrite Find.
-          * inv In. simpl_In.
-            eapply fresh_idents_rename_sub2 with (x:=k) in H0 as ((?&?&Find&_)&_). solve_In.
-            setoid_rewrite Find; simpl.
-            assert (FEnv.In (Var k) Hi') as (?&Hfind') by (apply H6, IsVar_senv_of_locs; eauto using In_InMembers).
-            esplit.
-            apply find_pred_snd_spec in Find; auto. rewrite Find; simpl; eauto.
-          * clear - In. destruct In as (?&Find). apply obind_inversion in Find as ((?&?)&Find&?).
-            apply Env.find_pred_spec in Find as (_&Eq). rewrite equiv_decb_equiv in Eq. inv Eq.
-          * clear - In. inv In. simpl_In. congruence.
-        +{ unfold st_senv. erewrite fresh_idents_rename_anns; eauto. split.
-           2:{ intros * _ Hla. exfalso. apply IsLast_app in Hla as [Hla|Hla].
-               - eapply Hnl, IsLast_app; eauto.
-               - apply senv_of_tyck_NoLast in Hla; auto.
-           }
-           destruct Hsc as (Hsc&_).
-           intros * Hck Hv; simpl in *.
-           unfold senv_of_tyck in Hck. simpl_app. rewrite Permutation_swap, HasClock_app in Hck.
-           apply sem_var_union in Hv.
-           assert (Hfresh:=H0). eapply fresh_idents_rename_ids in Hfresh; subst.
-           2:(erewrite fst_NoDupMembers, map_map, map_ext, <-fst_NoDupMembers; auto;
-              intros; destruct_conjs; auto).
-           assert (forall x, InMembers x locs -> ~ FEnv.In (Var x) Hi2) as Hdisj3.
-           { intros ? Hinm Henv. eapply Hdom in Henv.
-             apply IsVar_app in Henv as [Hin'|Hin'].
-             - apply IsVar_fst in Hin'. take (forall x, InMembers x locs -> ~_) and eapply it...
-             - eapply st_valid_AtomOrGensym_nIn with (st:=st); eauto using local_not_in_switch_prefs.
-               + eapply Forall_forall in H9...
-               + clear - Hin'. inv Hin'. solve_In. }
-           assert (forall x3, FEnv.In x3 Hi2 -> ~ FEnv.In x3 Hi') as Hdisj4.
-           { intros * In1 In2. destruct x4.
-             - eapply Hdisj3 in In1; eauto. now apply IsVar_senv_of_locs, H6.
-             - apply H6 in In2. clear - In2 H2. inv In2. simpl_In. simpl_Forall. subst; simpl in *; congruence. }
-           destruct Hck as [Hck|Hck], Hv as [Hv|Hv].
-           - exfalso. apply sem_var_In, Hdisj2 in Hv.
-             eapply Hv. inv Hck. simpl_In.
-             assert (FEnv.In (Var k) Hi') as [? Hfind'] by (eapply H6, IsVar_senv_of_locs; eauto using In_InMembers).
-             apply In_InMembers, Hsubin' in Hin as [? Hfind].
-             rewrite Hfind; simpl. econstructor; simpl.
-             erewrite find_pred_snd_spec; eauto.
-           - inv Hck. simpl_In.
-             assert (FEnv.In (Var k) Hi') as [vs Hfind'] by (eapply H6, IsVar_senv_of_locs; eauto using In_InMembers).
-             assert (sem_var Hi' (Var k) vs) as Hv' by (econstructor; eauto; reflexivity).
-             take (sc_vars _ _ _) and destruct it as (Hsc2&_).
-             eapply rename_var_sem in Hv' as Heq. eapply sem_var_det in Heq; [|apply Hv]. rewrite Heq.
-             eapply sem_var_refines, Hsc2 in Hv'; eauto using FEnv.union_refines4', EqStrel_Reflexive.
-             2:econstructor; solve_In; reflexivity.
-             simpl in *.
+          eapply Hnd'; eauto.
+          rewrite 2 in_app_iff, <-IsVar_fst; auto.
+        + rewrite app_assoc. eapply NoDupScope_NoDupMembers; eauto.
+          intros * InM1 In2. eapply Hnd'; eauto.
+          rewrite app_assoc, <-map_app, in_app_iff; auto.
+        + simpl_app. simpl_Forall.
+          eapply NoDupLocals_incl'. 4:eauto. all:eauto using local_not_in_switch_prefs.
+          intros *. repeat rewrite in_app_iff.
+          intros [|[|[In|[In|In]]]]; auto.
+          * clear - In. simpl_In. left. right. right. right. solve_In.
+          * clear - H0 H11 In. simpl_In.
+            eapply reuse_idents_find in H0 as (?&?&?&Reu&Find); eauto using In_InMembers.
+            unfold rename_var. erewrite Env.union_find3'; eauto. simpl.
+            eapply reuse_ident_gensym in Reu as [|]; subst; eauto.
+            left. right. right. right. solve_In.
+        + rewrite app_assoc. eapply local_hist_dom_ub; eauto.
+        + rewrite app_assoc, <-(@Typing.senv_of_locs_senv_of_anns exp).
+          eapply local_hist_dom; eauto. now rewrite Typing.senv_of_locs_senv_of_anns.
+        + rewrite app_assoc, <-(@Typing.senv_of_locs_senv_of_anns exp).
+          eapply local_hist_sc_vars; eauto using dom_dom_ub. reflexivity.
+          *{ intros * In1 In2. apply IsVar_fst in In2. simpl_In.
+             eapply reuse_idents_find' in H0 as (?&?&?&V1&Fol1&Fol2&Reu&Find); eauto using In_InMembers.
+             unfold rename_var in Hin. erewrite Env.union_find3' in Hin; [|eauto]. simpl in *. simpl_Forall.
+             eapply reuse_ident_st_nIn in Reu as Nin; eauto.
+             eapply Nin; eauto using st_follows_In. }
+          * now rewrite Typing.senv_of_locs_senv_of_anns.
+          *{ split.
+             2:{ intros * _ La. inv La. simpl_In. congruence. }
+
+             assert (forall x, InMembers x locs -> ~FEnv.In (Var x) Hi2) as Hdisj3.
+             { intros ? Hinm Henv. eapply Hdom in Henv.
+               eapply Hnd'; eauto.
+               rewrite <-2 map_app, <-IsVar_fst, 2 IsVar_app. apply IsVar_app in Henv as [|]; auto. }
+             assert (forall x3, FEnv.In x3 Hi2 -> ~ FEnv.In x3 Hi') as Hdisj4.
+             { intros * In1 In2. destruct x3.
+               - eapply Hdisj3 in In1; eauto. now apply IsVar_senv_of_locs, H6.
+               - apply H6 in In2. clear - In2 H2. inv In2. simpl_In. simpl_Forall. subst; simpl in *; congruence. }
+
+             intros * Ck Var. inv Ck. simpl_In.
+
+             take (sc_vars (senv_of_locs _) _ _) and destruct it as (Hsc2&_).
+             rewrite <-disjoint_union_rename_in_clock; auto.
              eapply subclock_clock_sem, subclock_clock_sem
-               with (Hi':= var_history (Hi2 + Hi')). 3,6:constructor; reflexivity. 5:eauto.
+               with (Hi':= var_history (Hi2 + _)). 3,6:constructor; reflexivity.
              + intros * Hs Hvar. rewrite sem_var_history in *.
                apply sem_var_union in Hvar as [Hvar|Hvar].
                * exfalso. eapply Hdisj3; eauto using sem_var_In.
                  apply Hsubin'. econstructor; eauto.
                * inv Hvar. econstructor; eauto.
-                 eapply FEnv.union3'. erewrite find_pred_snd_spec; eauto.
+                 eapply FEnv.union3'. erewrite find_snd_spec; eauto using reuse_idents_NoDup, Env.from_list_find_In.
              + intros * Hs Hvar. rewrite sem_var_history in *.
                apply sem_var_union in Hvar as [Hvar|Hvar].
                * apply sem_var_disj_union; eauto.
@@ -495,8 +524,8 @@ Module Type ILCORRECTNESS
              + intros * Hs Hvar. rewrite sem_var_history in *.
                apply sem_var_union in Hvar as [Hvar|Hvar].
                * eapply sem_var_disj_union; eauto.
-               * exfalso. apply sem_var_In, H6, IsVar_senv_of_locs, H13 in Hvar.
-                 eapply Hvar, in_app_iff, or_intror, IsVar_fst, Hsubin. econstructor; eauto.
+               * exfalso. apply sem_var_In, H6, IsVar_senv_of_locs, Hnd' in Hvar.
+                 eapply Hvar. rewrite 2 in_app_iff. right; left. apply IsVar_fst, Hsubin. econstructor; eauto.
              + intros * Hs Hvar. rewrite sem_var_history in *.
                apply sem_var_union in Hvar as [Hvar|Hvar].
                * eapply sem_var_disj_union; eauto.
@@ -504,134 +533,35 @@ Module Type ILCORRECTNESS
                  apply sem_var_In, Hub, IsVar_app in Hvar as [|Hvar]; auto with datatypes.
                  apply Hsubin, Env.Props.P.F.in_find_iff in Hvar. contradiction.
                * eapply sem_var_disj_union; eauto.
-             + intros * Hfind Hvar. inv Hvar. econstructor; eauto.
-               erewrite find_pred_snd_spec; eauto.
-             + intros * Hfind Hvar. exfalso.
-               eapply Env.Props.P.F.not_find_in_iff; eauto.
-               eapply Hsubin', IsVar_senv_of_locs, H6, sem_var_In; eauto.
-           - eapply sem_clock_refines; eauto using var_history_refines.
-           - exfalso.
-             eapply Hdisj2, sem_var_In, Hv.
-             apply Hdom. eauto with senv.
-         }
-    Qed.
-
-    Lemma inlinelocal_topblock_sem Γ : forall blk blks' locs' st st' bs Hi1 Hi2,
-        (forall x, ~IsLast Γ x) ->
-        (forall x vs, IsVar Γ x -> sem_var Hi1 (Var x) vs -> sem_var Hi2 (Var x) vs) ->
-        NoDupMembers Γ ->
-        noswitch_block blk ->
-        NoDupLocals (map fst Γ) blk ->
-        Forall (AtomOrGensym switch_prefs) (map fst Γ) ->
-        GoodLocals switch_prefs blk ->
-        wc_env (idck Γ) ->
-        wc_block G1 Γ blk ->
-        dom Hi1 Γ ->
-        sem_block_ck G1 Hi1 bs blk ->
-        dom Hi2 (Γ ++ st_senv st) ->
-        sc_vars (Γ++st_senv st) Hi2 bs ->
-        inlinelocal_topblock blk st = (blks', locs', st') ->
-        exists Hi3,
-          Hi2 ⊑ Hi3 /\
-          dom Hi3 ((Γ++senv_of_locs locs')++st_senv st') /\
-          sc_vars (Γ++senv_of_locs locs'++st_senv st') Hi3 bs /\
-          Forall (sem_block_ck G2 Hi3 bs) blks'.
-    Proof with eauto with datatypes.
-      Opaque inlinelocal_block.
-      destruct blk; intros * Hnl Hinm Hnd1 Hns Hnd2 Hatgen Hgood Hwenv Hwc Hdom1 Hsem Hdom2 Hsc Hil;
-        try destruct s; repeat inv_bind; simpl in *.
-      3:inv Hns.
-      1-3:eapply inlinelocal_block_sem with (Hi1:=Hi1) in H as (Hi3&?&Hdom3&Hsc3&?);
-        repeat rewrite app_nil_r in *; eauto; simpl in *.
-      16:inv Hns; inv Hnd2; inv Hgood; inv Hwc; inv Hsem; repeat inv_scope.
-      16:assert (forall x, FEnv.In x Hi2 -> ~FEnv.In x Hi') as Hdisj2.
-      16:{ intros * Hin2 Hin1. destruct x0; apply H4 in Hin1; apply Hdom2 in Hin2.
-           2:{ clear - Hin1 H2. inv Hin1. simpl_In. simpl_Forall. subst; simpl in *; congruence. }
-           apply IsVar_senv_of_locs in Hin1.
-           apply IsVar_app in Hin2 as [Hin2|Hin2]...
-           - apply IsVar_fst in Hin2. take (forall x, InMembers x _ -> ~In _ _) and eapply it; eauto.
-           - eapply st_valid_AtomOrGensym_nIn; eauto using local_not_in_switch_prefs.
-             eapply Forall_forall in H5...
-             clear - Hin2. inv Hin2; solve_In. }
-      16:assert (Hi1 + Hi' ⊑ Hi2 + Hi') as Href.
-      16:{ intros ?? Hv. apply FEnv.union4 in Hv as [Hv|Hv].
-           - destruct x0. 2:{ eapply FEnv.find_In, Hdom1, Hnl in Hv as []. }
-             assert (IsVar Γ x0) as Hin by (eapply Hdom1; econstructor; eauto).
-             assert (sem_var Hi2 (Var x0) v) as Hv2.
-             { eapply Hinm; [|econstructor; eauto; reflexivity]. now inv Hin. }
-             inv Hv2. do 2 esplit; eauto. apply FEnv.union2; auto.
-             apply FEnv.not_find_In. intros contra. apply H4, IsVar_senv_of_locs in contra.
-             take (forall x, InMembers x _ -> ~In _ _) and eapply it; eauto. now apply IsVar_fst.
-           - do 2 esplit; [reflexivity|auto using FEnv.union3'].
-      }
-      16:assert (Hi2 ⊑ Hi2 + Hi') as Href2.
-      16:{ intros ?? Hfind. do 2 esplit; try reflexivity.
-           apply FEnv.union2; auto.
-           apply FEnv.not_find_In, Hdisj2. econstructor; eauto. }
-      16:eapply mmap_inlinelocal_block_sem
-        with (Γ:=Γ++senv_of_locs locs')
-             (Hi1:=Hi1 + Hi')
-             (Hi2:=Hi2 + Hi')
-        in H as (Hi3&?&Hdom3&Hsc3&?);
-        repeat rewrite app_nil_r in *; eauto; simpl in *.
-      17:eapply Forall_forall; intros; eauto using inlinelocal_block_sem.
-      all:match goal with
-          | |- forall x, _ -> ~ IsVar [] x =>
-              intros * _ In; inv In; take (InMembers _ []) and inv it
-          | |- forall x, Env.In x (Env.empty ident) <-> _ =>
-              intros ?; rewrite Env.Props.P.F.empty_in_iff; split; [intros []|intros In]; inv In; take (InMembers _ []) and inv it
-          | |- forall x y vs, Env.find _ (Env.empty ident) = Some _ -> _ =>
-              intros * Hfind; eapply Env.Props.P.F.empty_mapsto_iff in Hfind as []
-          | |- forall x y, Env.MapsTo _ _ (Env.empty ident) -> _ =>
-              intros * Hfind; eapply Env.Props.P.F.empty_mapsto_iff in Hfind as []
-          | _ => idtac
-          end; auto using dom_dom_ub.
-      - exists Hi3. repeat (split; eauto).
-        + etransitivity; eauto using FEnv.union_refines4', EqStrel.
-        + clear - Hsc3. destruct Hsc3 as (Hsc3&_). simpl_app; eauto.
-        + clear - Hsc3. destruct Hsc3 as (_&Hsc3). simpl_app; eauto.
-      - rewrite NoLast_app; split; auto.
-        intros * Hla. inv Hla. simpl_In. simpl_Forall. subst; simpl in *; congruence.
-      - intros * Hinm1 Hv.
-        eapply sem_var_refines; [eapply Href|eauto].
-      - apply NoDupMembers_app; auto.
-        + apply NoDupMembers_senv_of_locs; auto.
-        + intros ? Hinm1 Hinm2. rewrite InMembers_senv_of_locs in Hinm2.
-          take (forall x, InMembers x _ -> ~In _ _) and eapply it...
-      - now rewrite map_app, map_fst_senv_of_locs.
-      - rewrite map_app, map_fst_senv_of_locs.
-        apply Forall_app; auto.
-      - unfold wc_env in *. simpl_app.
-        apply Forall_app; split; simpl_Forall; eauto.
-        eapply wc_clock_incl; eauto; solve_incl_app.
-      - eapply dom_dom_ub, local_hist_dom; eauto.
-      - unfold dom. rewrite <-app_assoc. setoid_rewrite (Permutation_app_comm (senv_of_locs _)). rewrite app_assoc.
-        eapply local_hist_dom; eauto.
-      - split.
-        2:{ intros * _ Hla. exfalso. repeat rewrite IsLast_app in Hla. destruct Hla as [[Hla|Hla]|Hla].
-            - eapply Hnl; eauto.
-            - inv Hla. simpl_In. simpl_Forall. subst; simpl in *; congruence.
-            - eapply senv_of_tyck_NoLast; eauto.
-        }
-        intros * Hck Hv. rewrite (Permutation_app_comm Γ), <-app_assoc, HasClock_app in Hck. destruct Hck as [Hck|Hck].
-        + edestruct H17 as (Hsc1&_).
-          eapply sem_clock_refines, Hsc1, sem_var_refines'; eauto using var_history_refines. simpl.
-          apply FEnv.union_In, or_intror, H4. inv Hck. econstructor. solve_In.
-        + destruct Hsc as (Hsc1&_).
-          eapply sem_clock_refines, Hsc1, sem_var_refines'; eauto using var_history_refines.
-          apply Hdom2. inv Hck. unfold st_ids, st_senv in *.
-          apply IsVar_app. apply in_app_iff in H0 as [|]; [left|right]; econstructor; eauto using In_InMembers.
-      Transparent inlinelocal_block.
+             + eapply Hsc2; eauto. econstructor; solve_In. auto.
+               assert (Reus:=H0). eapply reuse_idents_find in H0 as (?&?&?&Reu&Find); eauto using In_InMembers.
+               unfold rename_var in Var.
+               erewrite Env.union_find3' in Var; eauto. simpl in *.
+               apply sem_var_union in Var as [Var|Var].
+               * exfalso. eapply sem_var_In, Hdisj2 in Var.
+                 eapply Var; eauto using in_combine_r, Env.from_list_find_In.
+               * eapply sem_var_union3'. inv Var.
+                 apply obind_inversion in H0 as ((?&?)&Find'&?).
+                 erewrite find_snd_spec in Find'; eauto using reuse_idents_NoDup, Env.from_list_find_In. inv Find'.
+                 econstructor; eauto.
+           }
+        + eauto using reuse_idents_st_valid.
+        + rewrite app_assoc, map_app, Forall_app. split.
+          * simpl_Forall. eapply mmap_st_follows in H0; eauto using st_follows_In.
+            simpl_Forall; eauto using reuse_ident_st_follows.
+          * simpl_Forall. simpl_In.
+            eapply reuse_idents_find_follows in H0 as (?&?&?&Fol1&Fol2&Reu&Find); eauto using In_InMembers.
+            unfold rename_var. erewrite Env.union_find3'; eauto. simpl.
+            eapply reuse_ident_st_In in Reu; eauto using st_follows_In.
     Qed.
 
     Lemma inlinelocal_node_sem : forall f n ins outs,
-        wc_global (Global G1.(types) G1.(externs) (n::G1.(nodes))) ->
         Ordered_nodes (Global G1.(types) G1.(externs) (n::G1.(nodes))) ->
         Ordered_nodes (Global G2.(types) G2.(externs) ((inlinelocal_node n)::G2.(nodes))) ->
         sem_node_ck (Global G1.(types) G1.(externs) (n::G1.(nodes))) f ins outs ->
         sem_node_ck (Global G2.(types) G2.(externs) ((inlinelocal_node n)::G2.(nodes))) f ins outs.
     Proof with eauto.
-      intros * Hwc Hord1 Hord2 Hsem.
+      intros * Hord1 Hord2 Hsem.
 
       inv Hsem; rename H0 into Hfind; simpl in Hfind. destruct (ident_eq_dec (n_name n) f).
       - erewrite find_node_now in Hfind; eauto. inv Hfind.
@@ -642,38 +572,34 @@ Module Type ILCORRECTNESS
         replace {| types := types G1; nodes := nodes G1 |} with G1 in Hblksem by (destruct G1; auto).
         pose proof (n_nodup n0) as (Hnd1&Hnd2).
         pose proof (n_good n0) as (Hgood1&Hgood2&_).
-        inv Hwc. destruct H4 as (Hwc&_); simpl in Hwc.
         destruct H5 as (Hdom1&Hsc1).
-        eapply inlinelocal_topblock_sem
-          with (Γ:=senv_of_inout (n_in n0 ++ n_out n0))
-               (st:=init_st)
-               (Hi2:=H)
-               (blks':=fst (fst (inlinelocal_topblock (n_block n0) init_st)))
-               (locs':=snd (fst (inlinelocal_topblock (n_block n0) init_st)))
-               (st':=snd (inlinelocal_topblock (n_block n0) init_st))
-          in Hblksem as (Hf&Href&Hdom&Hsc&Hsem); eauto. 11:destruct inlinelocal_topblock as ((?&?)&?); reflexivity.
-        eapply Snode with (H:=H); simpl; eauto.
+        destruct (inlinelocal_block
+                    (Env.empty _) (n_block n0)
+                    {| fresh_st := Fresh.init_st; used := PSP.of_list (map fst (n_in n0 ++ n_out n0))|})
+          as ((locs'&blks')&st') eqn:Il. assert (Il':=Il).
+        eapply inlinelocal_block_sem
+                 with (Γ:=senv_of_inout (n_in n0 ++ n_out n0)) (Γ':=[]) (Γ'':=[])
+          in Il' as (Hf&Href&Hdom&Hsc&Hsem); repeat rewrite app_nil_r; eauto.
+        econstructor; eauto.
         + erewrite find_node_now; eauto.
         + eauto.
         + eauto.
         + apply sem_block_ck_cons'; simpl...
           2:{ eapply find_node_not_Is_node_in in Hord2.
             2:erewrite find_node_now; eauto. eauto. }
-          destruct (inlinelocal_topblock _ _) as ((?&?)&?) eqn:Hil.
-          assert (FEnv.Equiv (@EqSt _) Hf (H + restrict Hf (senv_of_locs l0 ++ st_senv f))) as Heq.
+          assert (FEnv.Equiv (@EqSt _) Hf (H + restrict Hf (senv_of_anns locs'))) as Heq.
           { intros ?. destruct (Hf x) eqn:Hfind.
-            - unfold restrict, FEnv.restrict. destruct (existsb (fun y : lustre_var => y ==b x) (vars_of_senv (senv_of_locs l0 ++ st_senv f))) eqn:Ex.
+            - unfold restrict, FEnv.restrict. destruct (existsb (fun y : lustre_var => y ==b x) (vars_of_senv (senv_of_anns locs'))) eqn:Ex.
               + erewrite FEnv.union3'; eauto using FEnv.restrict_find. 2:setoid_rewrite Ex; eauto.
                 reflexivity.
               + assert (FEnv.In x H) as (?&Hfind').
                 { destruct Hdom as (D2&DL2). apply FEnv.find_In in Hfind.
                   apply existsb_Forall, forallb_Forall, Forall_flat_map in Ex.
                   destruct x; apply Hdom1; [apply D2 in Hfind|apply DL2 in Hfind].
-                  1,2:rewrite <-app_assoc in Hfind. 1:apply IsVar_app in Hfind as [|Hfind]; auto. 2:apply IsLast_app in Hfind as [|Hfind]; auto.
-                  - inv Hfind. simpl_In. simpl_Forall.
+                  1,2:simpl in *. apply IsVar_app in Hfind as [|Hfind]; auto. 2:apply IsLast_app in Hfind as [|Hfind]; auto.
+                  - inv Hfind. simpl_In. unfold senv_of_anns in *. simpl_Forall.
                     rewrite equiv_decb_refl in H4. inv H4.
-                  - inv Hfind. simpl_Forall. destruct (causl_last _); try congruence. simpl in *; simpl_Forall.
-                    rewrite equiv_decb_refl in H9. inv H9.
+                  - inv Hfind. simpl_Forall. simpl_In. congruence.
                 }
                 assert (Hfind'':=Hfind'). apply Href in Hfind'' as (?&?&Hfind''). rewrite Hfind in Hfind''; inv Hfind''.
                 erewrite FEnv.union2; eauto using FEnv.restrict_find_None1.
@@ -682,36 +608,34 @@ Module Type ILCORRECTNESS
             - replace ((_ + _) x) with (@None (Stream svalue)); [constructor|].
               symmetry. apply FEnv.union_None; split; eauto using FEnv.restrict_find_None2, FEnv.refines_None.
           }
-          econstructor. eapply Sscope with (Hi':=restrict Hf (senv_of_locs l0 ++ st_senv f)).
+          rewrite Il in *. simpl in *.
+          econstructor. eapply Sscope with (Hi':=restrict Hf (senv_of_anns locs')).
           *{ destruct Hdom as (D&DL). split; intros *; unfold restrict.
-             1,2:rewrite FEnv.restrict_In, senv_of_locs_app.
-             - rewrite D, vars_of_senv_Var, 4 IsVar_app.
+             1,2:rewrite FEnv.restrict_In.
+             - rewrite D, vars_of_senv_Var, IsVar_app, Typing.senv_of_locs_senv_of_anns.
                split; intros; repeat (progress destruct_conjs || take (_ \/ _) and destruct it); auto.
-               1,2:right; clear - H3; inv H3; econstructor; solve_In.
-               clear - H0. split; right; inv H0; econstructor; unfold st_senv, senv_of_tyck; solve_In.
-             - rewrite DL, vars_of_senv_Last, 4 IsLast_app.
+             - rewrite DL, vars_of_senv_Last, IsLast_app, Typing.senv_of_locs_senv_of_anns.
                split; intros; repeat (progress destruct_conjs || take (_ \/ _) and destruct it); auto.
-               1,2:right; clear - H3; inv H3; econstructor; solve_In; auto.
-               clear - H0. split; right; inv H0; econstructor; unfold st_senv, senv_of_tyck; solve_In; auto.
            }
-          * apply Forall_app; split; simpl_Forall; simpl_In; [|constructor].
-            apply inlinelocal_topblock_nolast in Hil; auto. 2:apply n_syn. simpl_Forall; subst; constructor.
+          * simpl_Forall. constructor.
           * eapply sc_vars_morph. 1,3:reflexivity. eauto.
-            eapply sc_vars_incl; [|eauto]. unfold st_senv, senv_of_locs, senv_of_tyck. repeat solve_incl_app.
+            eapply sc_vars_incl; [|eauto]. unfold senv_of_locs, senv_of_tyck. solve_incl_app.
             erewrite map_map, map_ext; [reflexivity|]. intros; destruct_conjs; auto.
           * destruct G2; simpl in *. simpl_Forall.
             eapply sem_block_ck_morph; eauto. reflexivity.
         + simpl. constructor; simpl; auto.
-        + apply senv_of_inout_NoLast.
+        + simpl. apply senv_of_inout_NoLast.
+        + intros * _ In. inv In. inv H0.
+        + intros ?. rewrite Env.Props.P.F.empty_in_iff. split; intros In; inv In. inv H0.
+        + intros * Find. unfold Env.MapsTo in Find. rewrite Env.gempty in Find. congruence.
+        + intros * Find. rewrite Env.gempty in Find. congruence.
         + apply NoDupMembers_map; auto. intros; destruct_conjs; auto.
         + apply n_syn.
         + now rewrite map_fst_senv_of_inout.
         + now rewrite map_fst_senv_of_inout.
-        + destruct Hwc as (?&?&?); auto. simpl_app; auto.
-          erewrite 2 map_map, map_ext, map_ext with (l:=n_out _); eauto. 1,2:intros; destruct_conjs; auto.
-        + destruct Hwc as (?&?&?), G1; auto.
-        + unfold st_senv; rewrite init_st_anns, app_nil_r...
-        + unfold st_senv. rewrite init_st_anns, app_nil_r...
+        + auto using dom_dom_ub.
+        + intros ? In. apply In_of_list in In. now simpl_Forall.
+        + simpl_Forall. right. apply In_of_list. solve_In.
       - erewrite find_node_other in Hfind; eauto.
         eapply sem_node_ck_cons'...
         destruct G2; apply HGref.
